revert :(

src/Init/Data/Iterators/Combinators/Monadic/FlatMap.lean
@@ -8,7 +8,6 @@ module
 prelude
 public import Init.Data.Iterators.Combinators.Monadic.FilterMap
 public import Init.Data.Option.Lemmas
-import Init.Control.Lawful.MonadAttach.Lemmas
 
 /-!
 # Monadic `flatMap` combinator
@@ -204,34 +203,50 @@ public def IterM.flatMap {α : Type w} {β : Type w} {α₂ : Type w}
 
 variable {α α₂ β : Type w} {m : Type w → Type w'}
 
+/-- The plausible-step predicate for `Flatten` iterators -/
+public inductive Flatten.IsPlausibleStep [Iterator α m (IterM (α := α₂) m β)] [Iterator α₂ m β] :
+    (it : IterM (α := Flatten α α₂ β m) m β) → (step : IterStep (IterM (α := Flatten α α₂ β m) m β) β) → Prop where
+  | outerYield : ∀ {it₁ it₁' it₂'}, it₁.IsPlausibleStep (.yield it₁' it₂') →
+      IsPlausibleStep (toIterM ⟨it₁, none⟩ m β) (.skip (toIterM ⟨it₁', some it₂'⟩ m β))
+  | outerSkip : ∀ {it₁ it₁'}, it₁.IsPlausibleStep (.skip it₁') →
+      IsPlausibleStep (toIterM ⟨it₁, none⟩ m β) (.skip (toIterM ⟨it₁', none⟩ m β))
+  | outerDone : ∀ {it₁}, it₁.IsPlausibleStep .done →
+      IsPlausibleStep (toIterM ⟨it₁, none⟩ m β) .done
+  | innerYield : ∀ {it₁ it₂ it₂' b}, it₂.IsPlausibleStep (.yield it₂' b) →
+      IsPlausibleStep (toIterM ⟨it₁, some it₂⟩ m β) (.yield (toIterM ⟨it₁, some it₂'⟩ m β) b)
+  | innerSkip : ∀ {it₁ it₂ it₂'}, it₂.IsPlausibleStep (.skip it₂') →
+      IsPlausibleStep (toIterM ⟨it₁, some it₂⟩ m β) (.skip (toIterM ⟨it₁, some it₂'⟩ m β))
+  | innerDone : ∀ {it₁ it₂}, it₂.IsPlausibleStep .done →
+      IsPlausibleStep (toIterM ⟨it₁, some it₂⟩ m β) (.skip (toIterM ⟨it₁, none⟩ m β))
+
 public instance Flatten.instIterator [Monad m] [Iterator α m (IterM (α := α₂) m β)] [Iterator α₂ m β] :
     Iterator (Flatten α α₂ β m) m β where
+  IsPlausibleStep := IsPlausibleStep
   step it :=
     match it with
     | ⟨it₁, none⟩ => do
-      match ← it₁.step with
-      | .yield it₁' it₂' =>
-          return .skip ⟨it₁', some it₂'⟩
-      | .skip it₁' =>
-          return .skip ⟨it₁', none⟩
-      | .done =>
-          return .done
+      match (← it₁.step).inflate with
+      | .yield it₁' it₂' h =>
+          pure <| .deflate <| .skip ⟨it₁', some it₂'⟩ (.outerYield h)
+      | .skip it₁' h =>
+          pure <| .deflate <| .skip ⟨it₁', none⟩ (.outerSkip h)
+      | .done h =>
+          pure <| .deflate <| .done (.outerDone h)
     | ⟨it₁, some it₂⟩ => do
-      match ← it₂.step with
-      | .yield it₂' c =>
-          return .yield ⟨it₁, some it₂'⟩ c
-      | .skip it₂' =>
-          return .skip ⟨it₁, some it₂'⟩
-      | .done =>
-          return .skip ⟨it₁, none⟩
+      match (← it₂.step).inflate with
+      | .yield it₂' c h =>
+          pure <| .deflate <| .yield ⟨it₁, some it₂'⟩ c (.innerYield h)
+      | .skip it₂' h =>
+          pure <| .deflate <| .skip ⟨it₁, some it₂'⟩ (.innerSkip h)
+      | .done h =>
+          pure <| .deflate <| .skip ⟨it₁, none⟩ (.innerDone h)
 
 section Finite
 
 variable {α : Type w} {α₂ : Type w} {β : Type w} {m : Type w → Type w'}
 
 variable (α m β) in
-def Rel [Monad m] [MonadAttach m] [Iterator α m (IterM (α := α₂) m β)] [Iterator α₂ m β]
-    [Finite α m] [Finite α₂ m] :
+def Rel [Monad m] [Iterator α m (IterM (α := α₂) m β)] [Iterator α₂ m β] [Finite α m] [Finite α₂ m] :
     IterM (α := Flatten α α₂ β m) m β → IterM (α := Flatten α α₂ β m) m β → Prop :=
   InvImage
     (Prod.Lex
@@ -239,26 +254,24 @@ def Rel [Monad m] [MonadAttach m] [Iterator α m (IterM (α := α₂) m β)] [It
       (Option.lt (InvImage IterM.TerminationMeasures.Finite.Rel IterM.finitelyManySteps)))
     (fun it => (it.internalState.it₁, it.internalState.it₂))
 
-theorem Flatten.rel_of_left [Monad m] [MonadAttach m] [Iterator α m (IterM (α := α₂) m β)]
-    [Iterator α₂ m β] [Finite α m] [Finite α₂ m] {it it'}
+theorem Flatten.rel_of_left [Monad m] [Iterator α m (IterM (α := α₂) m β)] [Iterator α₂ m β]
+    [Finite α m] [Finite α₂ m] {it it'}
     (h : it'.internalState.it₁.finitelyManySteps.Rel it.internalState.it₁.finitelyManySteps) :
     Rel α β m it' it :=
   Prod.Lex.left _ _ h
 
-theorem Flatten.rel_of_right₁ [Monad m] [MonadAttach m] [Iterator α m (IterM (α := α₂) m β)]
-    [Iterator α₂ m β] [Finite α m] [Finite α₂ m] {it₁ it₂ it₂'}
+theorem Flatten.rel_of_right₁ [Monad m] [Iterator α m (IterM (α := α₂) m β)] [Iterator α₂ m β]
+    [Finite α m] [Finite α₂ m] {it₁ it₂ it₂'}
     (h : (InvImage IterM.TerminationMeasures.Finite.Rel IterM.finitelyManySteps) it₂' it₂) :
     Rel α β m ⟨it₁, some it₂'⟩ ⟨it₁, some it₂⟩ := by
   refine Prod.Lex.right _ h
 
-theorem Flatten.rel_of_right₂ [Monad m] [MonadAttach m] [Iterator α m (IterM (α := α₂) m β)]
-    [Iterator α₂ m β] [Finite α m] [Finite α₂ m] {it₁ it₂} :
+theorem Flatten.rel_of_right₂ [Monad m] [Iterator α m (IterM (α := α₂) m β)] [Iterator α₂ m β]
+    [Finite α m] [Finite α₂ m] {it₁ it₂} :
     Rel α β m ⟨it₁, none⟩ ⟨it₁, some it₂⟩ :=
   Prod.Lex.right _ True.intro
 
-def Flatten.instFinitenessRelation
-    [Monad m] [MonadAttach m] [LawfulMonad m] [LawfulMonadAttach m]
-    [Iterator α m (IterM (α := α₂) m β)] [Iterator α₂ m β]
+instance [Monad m] [Iterator α m (IterM (α := α₂) m β)] [Iterator α₂ m β]
     [Finite α m] [Finite α₂ m] :
     FinitenessRelation (Flatten α α₂ β m) m where
   rel := Rel α β m
@@ -268,41 +281,27 @@ def Flatten.instFinitenessRelation
     · exact InvImage.wf _ WellFoundedRelation.wf
     · exact Option.wellFounded_lt <| InvImage.wf _ WellFoundedRelation.wf
   subrelation {it it'} h := by
-    obtain ⟨step, hs, h⟩ := h
-    simp only [IterM.IsPlausibleStep, Iterator.step] at h
-    split at h
-    · obtain ⟨step', hs', h⟩ := LawfulMonadAttach.canReturn_bind_imp' h
-      cases step', hs' using PlausibleIterStep.casesOn'
-      · cases LawfulMonadAttach.eq_of_canReturn_pure h
-        cases hs
-        apply Flatten.rel_of_left
-        exact IterM.TerminationMeasures.Finite.rel_of_yield ‹_›
-      · cases LawfulMonadAttach.eq_of_canReturn_pure h
-        cases hs
-        apply Flatten.rel_of_left
-        exact IterM.TerminationMeasures.Finite.rel_of_skip ‹_›
-      · cases LawfulMonadAttach.eq_of_canReturn_pure h
-        nomatch hs
-    · obtain ⟨step', hs', h⟩ := LawfulMonadAttach.canReturn_bind_imp' h
-      cases step', hs' using PlausibleIterStep.casesOn'
-      · cases LawfulMonadAttach.eq_of_canReturn_pure h
-        cases hs
-        apply Flatten.rel_of_right₁
-        exact IterM.TerminationMeasures.Finite.rel_of_yield ‹_›
-      · cases LawfulMonadAttach.eq_of_canReturn_pure h
-        cases hs
-        apply Flatten.rel_of_right₁
-        exact IterM.TerminationMeasures.Finite.rel_of_skip ‹_›
-      · cases LawfulMonadAttach.eq_of_canReturn_pure h
-        cases hs
-        apply Flatten.rel_of_right₂
+    obtain ⟨step, h, h'⟩ := h
+    cases h' <;> cases h
+    case outerYield =>
+      apply Flatten.rel_of_left
+      exact IterM.TerminationMeasures.Finite.rel_of_yield ‹_›
+    case outerSkip =>
+      apply Flatten.rel_of_left
+      exact IterM.TerminationMeasures.Finite.rel_of_skip ‹_›
+    case innerYield =>
+      apply Flatten.rel_of_right₁
+      exact IterM.TerminationMeasures.Finite.rel_of_yield ‹_›
+    case innerSkip =>
+      apply Flatten.rel_of_right₁
+      exact IterM.TerminationMeasures.Finite.rel_of_skip ‹_›
+    case innerDone =>
+      apply Flatten.rel_of_right₂
 
 @[no_expose]
-public instance Flatten.instFinite
-    [Monad m] [MonadAttach m] [LawfulMonad m] [LawfulMonadAttach m]
-    [Iterator α m (IterM (α := α₂) m β)] [Iterator α₂ m β]
+public instance [Monad m] [Iterator α m (IterM (α := α₂) m β)] [Iterator α₂ m β]
     [Finite α m] [Finite α₂ m] : Finite (Flatten α α₂ β m) m :=
-  .of_finitenessRelation instFinitenessRelation
+  .of_finitenessRelation instFinitenessRelationFlattenOfIterMOfFinite
 
 end Finite
 
@@ -311,8 +310,8 @@ section Productive
 variable {α : Type w} {α₂ : Type w} {β : Type w} {m : Type w → Type w'}
 
 variable (α m β) in
-def ProductiveRel [Monad m] [MonadAttach m] [Iterator α m (IterM (α := α₂) m β)] [Iterator α₂ m β]
-    [Finite α m] [Productive α₂ m] :
+def ProductiveRel [Monad m] [Iterator α m (IterM (α := α₂) m β)] [Iterator α₂ m β] [Finite α m]
+    [Productive α₂ m] :
     IterM (α := Flatten α α₂ β m) m β → IterM (α := Flatten α α₂ β m) m β → Prop :=
   InvImage
     (Prod.Lex
@@ -320,27 +319,24 @@ def ProductiveRel [Monad m] [MonadAttach m] [Iterator α m (IterM (α := α₂) 
       (Option.lt (InvImage IterM.TerminationMeasures.Productive.Rel IterM.finitelyManySkips)))
     (fun it => (it.internalState.it₁, it.internalState.it₂))
 
-theorem Flatten.productiveRel_of_left [Monad m] [MonadAttach m] [Iterator α m (IterM (α := α₂) m β)]
+theorem Flatten.productiveRel_of_left [Monad m] [Iterator α m (IterM (α := α₂) m β)]
     [Iterator α₂ m β] [Finite α m] [Productive α₂ m] {it it'}
     (h : it'.internalState.it₁.finitelyManySteps.Rel it.internalState.it₁.finitelyManySteps) :
     ProductiveRel α β m it' it :=
   Prod.Lex.left _ _ h
 
-theorem Flatten.productiveRel_of_right₁ [Monad m] [MonadAttach m]
-    [Iterator α m (IterM (α := α₂) m β)] [Iterator α₂ m β] [Finite α m] [Productive α₂ m]
-    {it₁ it₂ it₂'} (h : (InvImage IterM.TerminationMeasures.Productive.Rel IterM.finitelyManySkips) it₂' it₂) :
+theorem Flatten.productiveRel_of_right₁ [Monad m] [Iterator α m (IterM (α := α₂) m β)] [Iterator α₂ m β]
+    [Finite α m] [Productive α₂ m] {it₁ it₂ it₂'}
+    (h : (InvImage IterM.TerminationMeasures.Productive.Rel IterM.finitelyManySkips) it₂' it₂) :
     ProductiveRel α β m ⟨it₁, some it₂'⟩ ⟨it₁, some it₂⟩ := by
   refine Prod.Lex.right _ h
 
-theorem Flatten.productiveRel_of_right₂ [Monad m] [MonadAttach m]
-    [Iterator α m (IterM (α := α₂) m β)] [Iterator α₂ m β]
+theorem Flatten.productiveRel_of_right₂ [Monad m] [Iterator α m (IterM (α := α₂) m β)] [Iterator α₂ m β]
     [Finite α m] [Productive α₂ m] {it₁ it₂} :
     ProductiveRel α β m ⟨it₁, none⟩ ⟨it₁, some it₂⟩ :=
   Prod.Lex.right _ True.intro
 
-def Flatten.instProductivenessRelation
-    [Monad m] [MonadAttach m] [LawfulMonad m] [LawfulMonadAttach m]
-    [Iterator α m (IterM (α := α₂) m β)] [Iterator α₂ m β]
+instance [Monad m] [Iterator α m (IterM (α := α₂) m β)] [Iterator α₂ m β]
     [Finite α m] [Productive α₂ m] :
     ProductivenessRelation (Flatten α α₂ β m) m where
   rel := ProductiveRel α β m
@@ -350,42 +346,32 @@ def Flatten.instProductivenessRelation
     · exact InvImage.wf _ WellFoundedRelation.wf
     · exact Option.wellFounded_lt <| InvImage.wf _ WellFoundedRelation.wf
   subrelation {it it'} h := by
-    simp only [IterM.IsPlausibleSkipSuccessorOf, IterM.IsPlausibleStep, Iterator.step] at h
-    split at h
-    · obtain ⟨step, hs, h⟩ := LawfulMonadAttach.canReturn_bind_imp' h
-      cases step, hs using PlausibleIterStep.casesOn'
-      · cases LawfulMonadAttach.eq_of_canReturn_pure h
-        apply Flatten.productiveRel_of_left
-        exact IterM.TerminationMeasures.Finite.rel_of_yield ‹_›
-      · cases LawfulMonadAttach.eq_of_canReturn_pure h
-        apply Flatten.productiveRel_of_left
-        exact IterM.TerminationMeasures.Finite.rel_of_skip ‹_›
-      · nomatch LawfulMonadAttach.eq_of_canReturn_pure h
-    · obtain ⟨step, hs, h⟩ := LawfulMonadAttach.canReturn_bind_imp' h
-      cases step, hs using PlausibleIterStep.casesOn'
-      · nomatch LawfulMonadAttach.eq_of_canReturn_pure h
-      · cases LawfulMonadAttach.eq_of_canReturn_pure h
-        apply Flatten.productiveRel_of_right₁
-        exact IterM.TerminationMeasures.Productive.rel_of_skip ‹_›
-      · cases LawfulMonadAttach.eq_of_canReturn_pure h
-        apply Flatten.productiveRel_of_right₂
+    cases h
+    case outerYield =>
+      apply Flatten.productiveRel_of_left
+      exact IterM.TerminationMeasures.Finite.rel_of_yield ‹_›
+    case outerSkip =>
+      apply Flatten.productiveRel_of_left
+      exact IterM.TerminationMeasures.Finite.rel_of_skip ‹_›
+    case innerSkip =>
+      apply Flatten.productiveRel_of_right₁
+      exact IterM.TerminationMeasures.Productive.rel_of_skip ‹_›
+    case innerDone =>
+      apply Flatten.productiveRel_of_right₂
 
 @[no_expose]
-public instance Flatten.instProductive
-    [Monad m] [MonadAttach m] [LawfulMonad m] [LawfulMonadAttach m]
-    [Iterator α m (IterM (α := α₂) m β)] [Iterator α₂ m β]
+public instance [Monad m] [Iterator α m (IterM (α := α₂) m β)] [Iterator α₂ m β]
     [Finite α m] [Productive α₂ m] : Productive (Flatten α α₂ β m) m :=
-  .of_productivenessRelation instProductivenessRelation
+  .of_productivenessRelation instProductivenessRelationFlattenOfFiniteIterMOfProductive
 
 end Productive
 
-public instance Flatten.instIteratorCollect [Monad m] [MonadAttach m] [Monad n]
-    [Iterator α m (IterM (α := α₂) m β)]
+public instance Flatten.instIteratorCollect [Monad m] [Monad n] [Iterator α m (IterM (α := α₂) m β)]
     [Iterator α₂ m β] : IteratorCollect (Flatten α α₂ β m) m n :=
   .defaultImplementation
 
-public instance Flatten.instIteratorLoop [Monad m] [MonadAttach m] [Monad n] [MonadAttach n]
-    [Iterator α m (IterM (α := α₂) m β)] [Iterator α₂ m β] : IteratorLoop (Flatten α α₂ β m) m n :=
+public instance Flatten.instIteratorLoop [Monad m] [Monad n] [Iterator α m (IterM (α := α₂) m β)]
+    [Iterator α₂ m β] : IteratorLoop (Flatten α α₂ β m) m n :=
   .defaultImplementation
 
 end Std.Iterators
