src/Init/Data/Iterators/Combinators/FilterMap.lean
@@ -32,6 +32,147 @@ Several variants of these combinators are provided:
 
 namespace Std.Iterators
 
+-- We cannot use `inherit_doc` because the docstring for `IterM` states that a `MonadLiftT` instance
+-- is needed.
+/--
+*Note: This is a very general combinator that requires an advanced understanding of monads,
+dependent types and termination proofs. The variants `filterMap` and `filterMapM` are easier to use
+and sufficient for most use cases.*
+
+If `it` is an iterator, then `it.filterMapWithPostcondition f` is another iterator that applies a monadic
+function `f` to all values emitted by `it`. `f` is expected to return an `Option` inside the monad.
+If `f` returns `none`, then nothing is emitted; if it returns `some x`, then `x` is emitted.
+
+`f` is expected to return `PostconditionT n (Option _)`, where `n` is an arbitrary monad.
+The `PostconditionT` transformer allows the caller to intrinsically prove properties about
+`f`'s return value in the monad `n`, enabling termination proofs depending on the specific behavior
+of `f`.
+
+**Marble diagram (without monadic effects):**
+
+```text
+it                                ---a --b--c --d-e--⊥
+it.filterMapWithPostcondition     ---a'-----c'-------⊥
+```
+
+(given that `f a = pure (some a')`, `f c = pure (some c')` and `f b = f d = d e = pure none`)
+
+**Termination properties:**
+
+* `Finite` instance: only if `it` is finite
+* `Productive` instance: only if `it` is finite
+
+For certain mapping functions `f`, the resulting iterator will be finite (or productive) even though
+no `Finite` (or `Productive`) instance is provided. For example, if `f` never returns `none`, then
+this combinator will preserve productiveness. If `f` is an `ExceptT` monad and will always fail,
+then `it.filterMapWithPostcondition` will be finite even if `it` isn't. In the first case, consider
+using the `map`/`mapM`/`mapWithPostcondition` combinators instead, which provide more instances out of
+the box.
+
+In such situations, the missing instances can be proved manually if the postcondition bundled in
+the `PostconditionT n` monad is strong enough. If `f` always returns `some _`, a suitable
+postcondition is `fun x => x.isSome`; if `f` always fails, a suitable postcondition might be
+`fun _ => False`.
+
+**Performance:**
+
+For each value emitted by the base iterator `it`, this combinator calls `f` and matches on the
+returned `Option` value.
+-/
+@[always_inline, inline, expose]
+def Iter.filterMapWithPostcondition {α β γ : Type w} [Iterator α Id β] {m : Type w → Type w'}
+    [Monad m] (f : β → PostconditionT m (Option γ)) (it : Iter (α := α) β) :=
+  (letI : MonadLift Id m := ⟨pure⟩; it.toIterM.filterMapWithPostcondition f : IterM m γ)
+
+/--
+*Note: This is a very general combinator that requires an advanced understanding of monads,
+dependent types and termination proofs. The variants `filter` and `filterM` are easier to use and
+sufficient for most use cases.*
+
+If `it` is an iterator, then `it.filterWithPostcondition f` is another iterator that applies a monadic
+predicate `f` to all values emitted by `it` and emits them only if they are accepted by `f`.
+
+`f` is expected to return `PostconditionT n (ULift Bool)`, where `n` is an arbitrary monad.
+The `PostconditionT` transformer allows the caller to intrinsically prove properties about
+`f`'s return value in the monad `n`, enabling termination proofs depending on the specific behavior
+of `f`.
+
+**Marble diagram (without monadic effects):**
+
+```text
+it                             ---a--b--c--d-e--⊥
+it.filterWithPostcondition     ---a-----c-------⊥
+```
+
+(given that `f a = f c = pure true` and `f b = f d = d e = pure false`)
+
+**Termination properties:**
+
+* `Finite` instance: only if `it` is finite
+* `Productive` instance: only if `it` is finite`
+
+For certain mapping functions `f`, the resulting iterator will be finite (or productive) even though
+no `Finite` (or `Productive`) instance is provided. For example, if `f` is an `ExceptT` monad and
+will always fail, then `it.filterWithPostcondition` will be finite -- and productive -- even if `it`
+isn't.
+
+In such situations, the missing instances can be proved manually if the postcondition bundled in
+the `PostconditionT n` monad is strong enough. In the given example, a suitable postcondition might
+be `fun _ => False`.
+
+**Performance:**
+
+For each value emitted by the base iterator `it`, this combinator calls `f`.
+-/
+@[always_inline, inline, expose]
+def Iter.filterWithPostcondition {α β : Type w} [Iterator α Id β] {m : Type w → Type w'}
+    [Monad m] (f : β → PostconditionT m (ULift Bool)) (it : Iter (α := α) β) :=
+  (letI : MonadLift Id m := ⟨pure⟩; it.toIterM.filterWithPostcondition f : IterM m β)
+
+/--
+*Note: This is a very general combinator that requires an advanced understanding of monads,
+dependent types and termination proofs. The variants `map` and `mapM` are easier to use and
+sufficient for most use cases.*
+
+If `it` is an iterator, then `it.mapWithPostcondition f` is another iterator that applies a monadic
+function `f` to all values emitted by `it` and emits the result.
+
+`f` is expected to return `PostconditionT n _`, where `n` is an arbitrary monad.
+The `PostconditionT` transformer allows the caller to intrinsically prove properties about
+`f`'s return value in the monad `n`, enabling termination proofs depending on the specific behavior
+of `f`.
+
+**Marble diagram (without monadic effects):**
+
+```text
+it                          ---a --b --c --d -e ----⊥
+it.mapWithPostcondition     ---a'--b'--c'--d'-e'----⊥
+```
+
+(given that `f a = pure a'`, `f b = pure b'` etc.)
+
+**Termination properties:**
+
+* `Finite` instance: only if `it` is finite
+* `Productive` instance: only if `it` is productive
+
+For certain mapping functions `f`, the resulting iterator will be finite (or productive) even though
+no `Finite` (or `Productive`) instance is provided. For example, if `f` is an `ExceptT` monad and
+will always fail, then `it.mapWithPostcondition` will be finite even if `it` isn't.
+
+In such situations, the missing instances can be proved manually if the postcondition bundled in
+the `PostconditionT n` monad is strong enough. In the given example, a suitable postcondition might
+be `fun _ => False`.
+
+**Performance:**
+
+For each value emitted by the base iterator `it`, this combinator calls `f`.
+-/
+@[always_inline, inline, expose]
+def Iter.mapWithPostcondition {α β γ : Type w} [Iterator α Id β] {m : Type w → Type w'}
+    [Monad m] (f : β → PostconditionT m γ) (it : Iter (α := α) β) :=
+  (letI : MonadLift Id m := ⟨pure⟩; it.toIterM.mapWithPostcondition f : IterM m γ)
+
 /--
 If `it` is an iterator, then `it.filterMapM f` is another iterator that applies a monadic
 function `f` to all values emitted by `it`. `f` is expected to return an `Option` inside the monad.
