src/Init/Data/Iterators/Combinators/Monadic/Attach.lean
@@ -8,7 +8,6 @@ module
 prelude
 public import Init.Data.Iterators.Internal.Termination
 public import Init.Data.Iterators.Consumers.Loop
-import Init.Control.Lawful.MonadAttach.Lemmas
 
 public section
 
@@ -18,74 +17,82 @@ namespace Std.Iterators.Types
 Internal state of the `attachWith` combinator. Do not depend on its internals.
 -/
 @[unbox]
-structure Attach (α : Type w) (m : Type w → Type w') {β : Type w} [MonadAttach m] [Iterator α m β]
+structure Attach (α : Type w) (m : Type w → Type w') {β : Type w} [Iterator α m β]
     (P : β → Prop) where
   inner : IterM (α := α) m β
   invariant : ∀ out, inner.IsPlausibleIndirectOutput out → P out
 
-instance Attach.instIterator {α β : Type w} {m : Type w → Type w'} [Monad m] [MonadAttach m]
+@[always_inline, inline]
+def Attach.Monadic.modifyStep {α : Type w} {m : Type w → Type w'} {β : Type w} [Iterator α m β]
+    {P : β → Prop}
+    (it : IterM (α := Attach α m P) m { out : β // P out })
+    (step : it.internalState.inner.Step (α := α) (m := m)) :
+    IterStep (IterM (α := Attach α m P) m { out : β // P out })
+        { out : β // P out } :=
+  match step with
+  | .yield it' out h =>
+    .yield ⟨it', fun out ho => it.internalState.invariant out (.indirect ⟨_, rfl, h⟩ ho)⟩
+      ⟨out, it.internalState.invariant out (.direct ⟨_, h⟩)⟩
+  | .skip it' h =>
+    .skip ⟨it', fun out ho => it.internalState.invariant out (.indirect ⟨_, rfl, h⟩ ho)⟩
+  | .done _ => .done
+
+instance Attach.instIterator {α β : Type w} {m : Type w → Type w'} [Monad m]
     [Iterator α m β] {P : β → Prop} :
     Iterator (Attach α m P) m { out : β // P out } where
-  step it := (fun ⟨step, hs⟩ =>
-    match step with
-    | .yield it' out =>
-      .yield ⟨it', fun out ho => it.internalState.invariant out (.indirect ⟨_, rfl, hs⟩ ho)⟩
-        ⟨out, it.internalState.invariant out (.direct ⟨_, hs⟩)⟩
-    | .skip it' =>
-      .skip ⟨it', fun out ho => it.internalState.invariant out (.indirect ⟨_, rfl, hs⟩ ho)⟩
-    | .done => .done) <$> MonadAttach.attach it.internalState.inner.step
+  IsPlausibleStep it step := ∃ step', Monadic.modifyStep it step' = step
+  step it := (fun step => .deflate ⟨Monadic.modifyStep it step.inflate, step.inflate, rfl⟩) <$>
+      it.internalState.inner.step
 
-def Attach.instFinitenessRelation {α β : Type w} {m : Type w → Type w'}
-    [Monad m] [MonadAttach m] [LawfulMonad m] [LawfulMonadAttach m]
+def Attach.instFinitenessRelation {α β : Type w} {m : Type w → Type w'} [Monad m]
     [Iterator α m β] [Finite α m] {P : β → Prop} :
     FinitenessRelation (Attach α m P) m where
   rel := InvImage WellFoundedRelation.rel fun it => it.internalState.inner.finitelyManySteps
   wf := InvImage.wf _ WellFoundedRelation.wf
   subrelation {it it'} h := by
-    obtain ⟨_, hs, h⟩ := h
-    obtain ⟨step, h', rfl⟩ := LawfulMonadAttach.canReturn_map_imp' h
+    apply Relation.TransGen.single
+    obtain ⟨_, hs, step, h', rfl⟩ := h
     cases step using PlausibleIterStep.casesOn
-    · simp only [IterStep.successor, Option.some.injEq] at hs
+    · simp only [IterStep.successor, Monadic.modifyStep, Option.some.injEq] at hs
       simp only [← hs]
-      exact IterM.TerminationMeasures.Finite.rel_of_yield ‹_›
-    · simp only [IterStep.successor, Option.some.injEq] at hs
+      exact ⟨_, rfl, ‹_›⟩
+    · simp only [IterStep.successor, Monadic.modifyStep, Option.some.injEq] at hs
       simp only [← hs]
-      exact IterM.TerminationMeasures.Finite.rel_of_skip ‹_›
-    · simp [IterStep.successor, reduceCtorEq] at hs
+      exact ⟨_, rfl, ‹_›⟩
+    · simp [IterStep.successor, Monadic.modifyStep, reduceCtorEq] at hs
 
-instance Attach.instFinite {α β : Type w} {m : Type w → Type w'}
-    [Monad m] [MonadAttach m] [LawfulMonad m] [LawfulMonadAttach m]
+instance Attach.instFinite {α β : Type w} {m : Type w → Type w'} [Monad m]
     [Iterator α m β] [Finite α m] {P : β → Prop} : Finite (Attach α m P) m :=
   .of_finitenessRelation instFinitenessRelation
 
-def Attach.instProductivenessRelation {α β : Type w} {m : Type w → Type w'}
-    [Monad m] [MonadAttach m] [LawfulMonad m] [LawfulMonadAttach m]
+def Attach.instProductivenessRelation {α β : Type w} {m : Type w → Type w'} [Monad m]
     [Iterator α m β] [Productive α m] {P : β → Prop} :
     ProductivenessRelation (Attach α m P) m where
   rel := InvImage WellFoundedRelation.rel fun it => it.internalState.inner.finitelyManySkips
   wf := InvImage.wf _ WellFoundedRelation.wf
   subrelation {it it'} h := by
-    obtain ⟨step, h', h⟩ := LawfulMonadAttach.canReturn_map_imp' h
+    apply Relation.TransGen.single
+    simp_wf
+    obtain ⟨step, hs⟩ := h
     cases step using PlausibleIterStep.casesOn
-    · cases h
-    · cases h
-      exact IterM.TerminationMeasures.Productive.rel_of_skip ‹_›
-    · cases h
+    · simp [Monadic.modifyStep] at hs
+    · simp only [Monadic.modifyStep, IterStep.skip.injEq] at hs
+      simp only [← hs]
+      assumption
+    · simp [Monadic.modifyStep] at hs
 
-instance Attach.instProductive {α β : Type w} {m : Type w → Type w'}
-    [Monad m] [MonadAttach m] [LawfulMonad m] [LawfulMonadAttach m]
+instance Attach.instProductive {α β : Type w} {m : Type w → Type w'} [Monad m]
     [Iterator α m β] [Productive α m] {P : β → Prop} :
     Productive (Attach α m P) m :=
   .of_productivenessRelation instProductivenessRelation
 
-instance Attach.instIteratorCollect {α β : Type w} {m : Type w → Type w'}
-    [Monad m] [MonadAttach m] [Monad n]
+instance Attach.instIteratorCollect {α β : Type w} {m : Type w → Type w'} [Monad m] [Monad n]
     {P : β → Prop} [Iterator α m β] :
     IteratorCollect (Attach α m P) m n :=
   .defaultImplementation
 
-instance Attach.instIteratorLoop {α β : Type w} {m : Type w → Type w'} [Monad m] [MonadAttach m]
-    {n : Type x → Type x'} [Monad n] [MonadAttach n] {P : β → Prop} [Iterator α m β] :
+instance Attach.instIteratorLoop {α β : Type w} {m : Type w → Type w'} [Monad m]
+    {n : Type x → Type x'} [Monad n] {P : β → Prop} [Iterator α m β] :
     IteratorLoop (Attach α m P) m n :=
   .defaultImplementation
 
@@ -101,7 +108,7 @@ iterator with values in the corresponding subtype `{ x // P x }`.
 * `Productive` instance: only if the base iterator is productive
 -/
 @[always_inline, inline, expose]
-def IterM.attachWith {α β : Type w} {m : Type w → Type w'} [Monad m] [MonadAttach m]
+def IterM.attachWith {α β : Type w} {m : Type w → Type w'} [Monad m]
     [Iterator α m β] (it : IterM (α := α) m β) (P : β → Prop)
     (h : ∀ out, it.IsPlausibleIndirectOutput out → P out) :
     IterM (α := Types.Attach α m P) m { out : β // P out } :=
