src/Init/Data/Iterators/Combinators/Monadic/ULift.lean
@@ -8,7 +8,6 @@ module
 prelude
 public import Init.Data.Iterators.Internal.Termination
 public import Init.Data.Iterators.Consumers.Monadic
-import Init.Control.Lawful.MonadAttach.Lemmas
 
 public section
 
@@ -85,68 +84,51 @@ def Types.ULiftIterator.Monadic.modifyStep (step : IterStep (IterM (α := α) m 
 
 instance Types.ULiftIterator.instIterator [Iterator α m β] [Monad n] :
     Iterator (ULiftIterator α m n β lift) n (ULift β) where
+  IsPlausibleStep it step :=
+    ∃ step', it.internalState.inner.IsPlausibleStep step' ∧
+      step = ULiftIterator.Monadic.modifyStep step'
   step it := do
-    (Monadic.modifyStep ·.down) <$> (lift it.internalState.inner.step).run
+    let step := (← (lift it.internalState.inner.step).run).down
+    return .deflate ⟨Monadic.modifyStep step.inflate.val, ?hp⟩
+  where finally
+    case hp => exact ⟨step.inflate.val, step.inflate.property, rfl⟩
 
-def Types.ULiftIterator.instFinitenessRelation
-    [Monad m] [MonadAttach m] [LawfulMonad m] [LawfulMonadAttach m]
-    [Monad n] [LawfulMonad n] [MonadAttach n] [LawfulMonadAttach n]
-    [Iterator α m β] [Finite α m] [Internal.LawfulMonadLiftFunction lift] :
+def Types.ULiftIterator.instFinitenessRelation [Iterator α m β] [Finite α m] [Monad n] :
     FinitenessRelation (ULiftIterator α m n β lift) n where
   rel := InvImage WellFoundedRelation.rel (fun it => it.internalState.inner.finitelyManySteps)
   wf := InvImage.wf _ WellFoundedRelation.wf
-  subrelation {it it'} h := by
-    rcases h with ⟨_, hs, h⟩
-    simp only [IterM.IsPlausibleStep, Iterator.step, ← LawfulMonadAttach.map_attach (x := it.internalState.inner.step),
-      Internal.LawfulMonadLiftFunction.lift_map, ULiftT.run, instMonadULiftT] at h
-    simp only [Function.comp_apply, bind_pure_comp, Functor.map_map] at h
-    obtain ⟨⟨step⟩, hstep, rfl⟩ := LawfulMonadAttach.canReturn_map_imp' h
-    cases step using PlausibleIterStep.casesOn
-    · cases hs
-      exact IterM.TerminationMeasures.Finite.rel_of_yield ‹_›
-    · cases hs
-      exact IterM.TerminationMeasures.Finite.rel_of_skip ‹_›
-    · cases hs
+  subrelation h := by
+    rcases h with ⟨_, hs, step, hp, rfl⟩
+    cases step <;> cases hs
+    · apply IterM.TerminationMeasures.Finite.rel_of_yield
+      exact hp
+    · apply IterM.TerminationMeasures.Finite.rel_of_skip
+      exact hp
 
-instance Types.ULiftIterator.instFinite
-    [Monad m] [MonadAttach m] [LawfulMonad m] [LawfulMonadAttach m]
-    [Monad n] [LawfulMonad n] [MonadAttach n] [LawfulMonadAttach n]
-    [Iterator α m β] [Finite α m] [Internal.LawfulMonadLiftFunction lift] :
+instance Types.ULiftIterator.instFinite [Iterator α m β] [Finite α m] [Monad n] :
     Finite (ULiftIterator α m n β lift) n :=
   .of_finitenessRelation instFinitenessRelation
 
-def Types.ULiftIterator.instProductivenessRelation
-    [Monad m] [MonadAttach m] [LawfulMonad m] [LawfulMonadAttach m]
-    [Monad n] [LawfulMonad n] [MonadAttach n] [LawfulMonadAttach n]
-    [Iterator α m β] [Productive α m] [Internal.LawfulMonadLiftFunction lift] :
+def Types.ULiftIterator.instProductivenessRelation [Iterator α m β] [Productive α m] [Monad n] :
     ProductivenessRelation (ULiftIterator α m n β lift) n where
   rel := InvImage WellFoundedRelation.rel (fun it => it.internalState.inner.finitelyManySkips)
   wf := InvImage.wf _ WellFoundedRelation.wf
-  subrelation {it it'} h := by
-    simp only [IterM.IsPlausibleSkipSuccessorOf, IterM.IsPlausibleStep, Iterator.step, ← LawfulMonadAttach.map_attach (x := it.internalState.inner.step),
-      Internal.LawfulMonadLiftFunction.lift_map, ULiftT.run, instMonadULiftT] at h
-    simp only [Function.comp_apply, bind_pure_comp, Functor.map_map] at h
-    obtain ⟨⟨step⟩, hstep, h⟩ := LawfulMonadAttach.canReturn_map_imp' h
-    cases step using PlausibleIterStep.casesOn
-    · cases h
-    · cases h
-      exact IterM.TerminationMeasures.Productive.rel_of_skip ‹_›
-    · cases h
+  subrelation h := by
+    rcases h with ⟨step, hp, hs⟩
+    cases step <;> cases hs
+    apply IterM.TerminationMeasures.Productive.rel_of_skip
+    exact hp
 
-instance Types.ULiftIterator.instProductive
-    [Monad m] [MonadAttach m] [LawfulMonad m] [LawfulMonadAttach m]
-    [Monad n] [LawfulMonad n] [MonadAttach n] [LawfulMonadAttach n]
-    [Iterator α m β] [Productive α m] [Internal.LawfulMonadLiftFunction lift] :
+instance Types.ULiftIterator.instProductive [Iterator α m β] [Productive α m] [Monad n] :
     Productive (ULiftIterator α m n β lift) n :=
   .of_productivenessRelation instProductivenessRelation
 
-instance Types.ULiftIterator.instIteratorLoop {o : Type x → Type x'}
-    [Monad n] [MonadAttach n] [Monad o] [MonadAttach o] [Iterator α m β] :
+instance Types.ULiftIterator.instIteratorLoop {o : Type x → Type x'} [Monad n] [Monad o]
+    [Iterator α m β] :
     IteratorLoop (ULiftIterator α m n β lift) n o :=
   .defaultImplementation
 
-instance Types.ULiftIterator.instIteratorCollect
-    [Monad n] [MonadAttach n] [Monad o] [Iterator α m β] :
+instance Types.ULiftIterator.instIteratorCollect [Monad n] [Monad o] [Iterator α m β] :
     IteratorCollect (ULiftIterator α m n β lift) n o :=
   .defaultImplementation
 
