src/Init/Data/Iterators/Consumers/Monadic/Access.lean
@@ -17,8 +17,8 @@ namespace Std.Iterators
 `IsPlausibleStep` relation, it is plausible that `step` returns the step in which the `n`-th value
 of `it` is emitted, or `.done` if `it` can plausibly terminate before emitting `n` values.
 -/
-inductive IterM.IsPlausibleNthOutputStep {α β : Type w} {m : Type w → Type w'} [MonadAttach m]
-    [Iterator α m β] : Nat → IterM (α := α) m β → IterStep (IterM (α := α) m β) β → Prop where
+inductive IterM.IsPlausibleNthOutputStep {α β : Type w} {m : Type w → Type w'} [Iterator α m β] :
+    Nat → IterM (α := α) m β → IterStep (IterM (α := α) m β) β → Prop where
   /-- If `it` plausibly yields in its immediate next step, this step is a plausible `0`-th output step. -/
   | zero_yield {it : IterM (α := α) m β} : it.IsPlausibleStep (.yield it' out) →
       it.IsPlausibleNthOutputStep 0 (.yield it' out)
@@ -43,8 +43,8 @@ inductive IterM.IsPlausibleNthOutputStep {α β : Type w} {m : Type w → Type w
   | skip {it it' : IterM (α := α) m β} {step} : it.IsPlausibleStep (.skip it') →
       it'.IsPlausibleNthOutputStep n step → it.IsPlausibleNthOutputStep n step
 
-theorem IterM.not_isPlausibleNthOutputStep_skip {α β : Type w} {m : Type w → Type w'}
-    [MonadAttach m] [Iterator α m β] {n : Nat} {it it' : IterM (α := α) m β} :
+theorem IterM.not_isPlausibleNthOutputStep_yield {α β : Type w} {m : Type w → Type w'} [Iterator α m β]
+    {n : Nat} {it it' : IterM (α := α) m β} :
     ¬ it.IsPlausibleNthOutputStep n (.skip it') := by
   intro h
   generalize h' : IterStep.skip it' = step at h
@@ -66,16 +66,9 @@ is guaranteed to plausible in the sense of `IterM.IsPlausibleNthOutputStep`.
 
 This class is experimental and users of the iterator API should not explicitly depend on it.
 -/
-class IteratorAccess (α : Type w) (m : Type w → Type w') {β : Type w}
-    [Iterator α m β] where
+class IteratorAccess (α : Type w) (m : Type w → Type w') {β : Type w} [Iterator α m β] where
   nextAtIdx? (it : IterM (α := α) m β) (n : Nat) :
-    m (IterM.Step (α := α) m β)
-
-class LawfulIteratorAccess (α : Type w) (m : Type w → Type w') {β : Type w}
-    [MonadAttach m] [Iterator α m β] [IteratorAccess α m] where
-  isPlausibleNthOutputStep_of_canReturn {it : IterM (α := α) m β} {n : Nat} {s} :
-    MonadAttach.CanReturn (IteratorAccess.nextAtIdx? it n) s → it.IsPlausibleNthOutputStep n s
-  -- TODO: correctness
+    m (PlausibleIterStep (it.IsPlausibleNthOutputStep n))
 
 /--
 Returns the step in which `it` yields its `n`-th element, or `.done` if it terminates earlier.
@@ -91,7 +84,7 @@ the `IteratorAccess` typeclass.
 -/
 @[always_inline, inline]
 def IterM.nextAtIdx? [Iterator α m β] [IteratorAccess α m] (it : IterM (α := α) m β)
-    (n : Nat) : m (IterM.Step (α := α) m β) :=
+    (n : Nat) : m (PlausibleIterStep (it.IsPlausibleNthOutputStep n)) :=
   IteratorAccess.nextAtIdx? it n
 
 /--
@@ -105,9 +98,9 @@ This function is only available for iterators that explicitly support it by impl
 the `IteratorAccess` typeclass.
 -/
 @[always_inline, inline]
-def IterM.atIdx? [MonadAttach m] [Iterator α m β] [IteratorAccess α m] [Monad m]
-    (it : IterM (α := α) m β) (n : Nat) : m (Option β) := do
-  match ← IteratorAccess.nextAtIdx? it n with
+def IterM.atIdx? [Iterator α m β] [IteratorAccess α m] [Monad m] (it : IterM (α := α) m β)
+    (n : Nat) : m (Option β) := do
+  match (← IteratorAccess.nextAtIdx? it n).val with
   | .yield _ out => return some out
   | .skip _ => return none
   | .done => return none
