src/Init/Data/Iterators/Consumers/Stream.lean
@@ -8,24 +8,20 @@ module
 prelude
 public import Init.Data.Stream
 public import Init.Data.Iterators.Consumers.Access
-import all Init.Data.Iterators.Consumers.Monadic.Access
 
 public section
 
 namespace Std.Iterators
 
-instance {α β} [Iterator α Id β] [Productive α Id]
-    [IteratorAccess α Id] [LawfulIteratorAccess α Id] :
+instance {α β} [Iterator α Id β] [Productive α Id] [IteratorAccess α Id] :
     Stream (Iter (α := α) β) β where
-  next? it := match h : (it.toIterM.nextAtIdx? 0).run with
-    | .yield it' out => some (out, it'.toIter)
-    | .skip it' => False.elim ?noskip
-    | .done => none
+  next? it := match (it.toIterM.nextAtIdx? 0).run with
+    | .yield it' out _ => some (out, it'.toIter)
+    | .skip _ h => False.elim ?noskip
+    | .done _ => none
   where finally
     case noskip =>
       revert h
-      have := IterM.not_isPlausibleNthOutputStep_skip (α := α) (m := Id) (it := it.toIterM) (it' := it') (n := 0)
-      replace := this.imp LawfulIteratorAccess.isPlausibleNthOutputStep_of_canReturn
-      exact this
+      exact IterM.not_isPlausibleNthOutputStep_yield
 
 end Std.Iterators
