src/Init/Data/Iterators/Lemmas/Consumers/Monadic/Collect.lean
@@ -21,24 +21,19 @@ open Std.Internal
 variable {α β γ : Type w} {m : Type w → Type w'} {n : Type w → Type w''}
   {lift : ⦃δ : Type w⦄ → m δ → n δ} {f : β → n γ} {it : IterM (α := α) m β}
 
-private theorem IterM.DefaultConsumers.toArrayMapped.go_eq [Monad m] [Monad n]
-    [MonadAttach m] [MonadAttach n] [Iterator α m β] [Finite α m]
-    [LawfulMonad m] [LawfulMonadAttach m] [LawfulMonad n]
-    [LawfulMonadLiftFunction lift] {acc : Array γ} :
+private theorem IterM.DefaultConsumers.toArrayMapped.go_eq [Monad n]
+    [Iterator α m β] [LawfulMonad n] [Finite α m] {acc : Array γ} :
     letI : MonadLift m n := ⟨lift (δ := _)⟩
-    haveI : LawfulMonadLift m n := sorry
     go lift f it acc (m := m) = (do
-      match ← it.step with
+      match (← it.step).inflate.val with
       | .yield it' out => go lift f it' (acc.push (← f out))
       | .skip it' => go lift f it' acc
       | .done => return acc) := by
   letI : MonadLift m n := ⟨lift (δ := _)⟩
   rw [toArrayMapped.go, WellFounded.extrinsicFix₂_eq_apply]
   · simp only
-    conv => rhs; rw [← LawfulMonadAttach.map_attach (x := it.step)]
-    simp only [liftM_map, bind_map_left]
     apply bind_congr; intro step
-    cases step using PlausibleIterStep.casesOn
+    cases step.inflate using PlausibleIterStep.casesOn
     · apply bind_congr; intro fx
       simp [go]
     · simp [go]
@@ -47,28 +42,16 @@ private theorem IterM.DefaultConsumers.toArrayMapped.go_eq [Monad m] [Monad n]
     apply InvImage.wf
     exact WellFoundedRelation.wf
 
-private theorem IterM.DefaultConsumers.toArrayMapped.go.aux₁ [Monad m] [Monad n]
-    [MonadAttach m] [MonadAttach n] [LawfulMonad m] [LawfulMonad n]
-    [LawfulMonadAttach m] [LawfulMonadLiftFunction lift]
+private theorem IterM.DefaultConsumers.toArrayMapped.go.aux₁ [Monad n] [LawfulMonad n]
     [Iterator α m β] [Finite α m] {b : γ} {bs : Array γ} :
     IterM.DefaultConsumers.toArrayMapped.go lift f it (#[b] ++ bs) (m := m) =
       (#[b] ++ ·) <$> IterM.DefaultConsumers.toArrayMapped.go lift f it bs (m := m) := by
   induction it using IterM.inductSteps generalizing bs with | step it ihy ihs
   rw [go_eq, map_eq_pure_bind, go_eq, bind_assoc]
-  rw [← LawfulMonadAttach.map_attach (x := it.step)]
-  simp only [liftM_map, bind_map_left]
   apply bind_congr; intro step
-  cases step using PlausibleIterStep.casesOn
-  · simp only [bind_pure_comp, map_bind]
-    apply bind_congr
-    simp [ihy ‹_›]
-  · simp [ihs ‹_›]
-  · simp
+  cases step.inflate using PlausibleIterStep.casesOn <;> simp (discharger := assumption) [ihy, ihs]
 
-private theorem IterM.DefaultConsumers.toArrayMapped.go.aux₂
-    [Monad m] [MonadAttach m] [LawfulMonad m] [LawfulMonadAttach m]
-    [Monad n] [MonadAttach n] [LawfulMonad n]
-    [LawfulMonadLiftFunction lift]
+private theorem IterM.DefaultConsumers.toArrayMapped.go.aux₂ [Monad n] [LawfulMonad n]
     [Iterator α m β] [Finite α m] {acc : Array γ} :
     IterM.DefaultConsumers.toArrayMapped.go lift f it acc (m := m) =
       (acc ++ ·) <$> IterM.DefaultConsumers.toArrayMapped lift f it (m := m) := by
@@ -80,36 +63,30 @@ private theorem IterM.DefaultConsumers.toArrayMapped.go.aux₂
     rw [List.toArray_cons, IterM.DefaultConsumers.toArrayMapped.go.aux₁, ih]
     simp only [Functor.map_map, Array.append_assoc]
 
-theorem IterM.DefaultConsumers.toArrayMapped_eq_match_step
-    [Monad m] [MonadAttach m] [LawfulMonad m] [LawfulMonadAttach m]
-    [Monad n] [MonadAttach n] [LawfulMonad n]
-    [LawfulMonadLiftFunction lift]
+theorem IterM.DefaultConsumers.toArrayMapped_eq_match_step [Monad n] [LawfulMonad n]
     [Iterator α m β] [Finite α m] :
     IterM.DefaultConsumers.toArrayMapped lift f it (m := m) = letI : MonadLift m n := ⟨lift (δ := _)⟩; (do
-      match ← it.step with
+      match (← it.step).inflate.val with
       | .yield it' out =>
         return #[← f out] ++ (← IterM.DefaultConsumers.toArrayMapped lift f it' (m := m))
       | .skip it' => IterM.DefaultConsumers.toArrayMapped lift f it' (m := m)
       | .done => return #[]) := by
   rw [IterM.DefaultConsumers.toArrayMapped, IterM.DefaultConsumers.toArrayMapped.go_eq]
-  rw [← LawfulMonadAttach.map_attach (x := it.step)]
-  simp only [liftM_map, bind_map_left]
-  apply bind_congr; intro step
-  cases step using PlausibleIterStep.casesOn <;>
+  apply bind_congr
+  intro step
+  cases step.inflate using PlausibleIterStep.casesOn <;>
     simp [IterM.DefaultConsumers.toArrayMapped.go.aux₂]
 
 @[simp]
-theorem IterM.toArray_ensureTermination
-    [Monad m] [MonadAttach m] [LawfulMonad m] [LawfulMonadAttach m]
-    [Iterator α m β] [Finite α m] [IteratorCollect α m m] {it : IterM (α := α) m β} :
+theorem IterM.toArray_ensureTermination [Monad m] [Iterator α m β] [Finite α m]
+    [IteratorCollect α m m] {it : IterM (α := α) m β} :
     it.ensureTermination.toArray = it.toArray :=
   (rfl)
 
-theorem IterM.toArray_eq_match_step
-    [Monad m] [MonadAttach m] [LawfulMonad m] [LawfulMonadAttach m]
-    [Iterator α m β] [Finite α m] [IteratorCollect α m m] [LawfulIteratorCollect α m m] :
+theorem IterM.toArray_eq_match_step [Monad m] [LawfulMonad m] [Iterator α m β] [Finite α m]
+    [IteratorCollect α m m] [LawfulIteratorCollect α m m] :
     it.toArray = (do
-      match ← it.step with
+      match (← it.step).inflate.val with
       | .yield it' out => return #[out] ++ (← it'.toArray)
       | .skip it' => it'.toArray
       | .done => return #[]) := by
@@ -117,59 +94,47 @@ theorem IterM.toArray_eq_match_step
   rw [IterM.DefaultConsumers.toArrayMapped_eq_match_step]
   simp [bind_pure_comp, pure_bind]
 
-theorem IterM.toArray_ensureTermination_eq_match_step
-    [Monad m] [MonadAttach m] [LawfulMonad m] [LawfulMonadAttach m]
-    [Iterator α m β] [Finite α m] [IteratorCollect α m m] [LawfulIteratorCollect α m m] :
+theorem IterM.toArray_ensureTermination_eq_match_step [Monad m] [LawfulMonad m] [Iterator α m β]
+    [Finite α m] [IteratorCollect α m m] [LawfulIteratorCollect α m m] :
     it.ensureTermination.toArray = (do
-      match ← it.step with
+      match (← it.step).inflate.val with
       | .yield it' out => return #[out] ++ (← it'.toArray)
       | .skip it' => it'.toArray
       | .done => return #[]) := by
   rw [toArray_ensureTermination, toArray_eq_match_step]
 
 @[simp]
-theorem IterM.toList_ensureTermination
-    [Monad m] [MonadAttach m] [LawfulMonad m] [LawfulMonadAttach m]
-    [Iterator α m β] [Finite α m] [IteratorCollect α m m] {it : IterM (α := α) m β} :
+theorem IterM.toList_ensureTermination [Monad m] [Iterator α m β] [Finite α m]
+    [IteratorCollect α m m] {it : IterM (α := α) m β} :
     it.ensureTermination.toList = it.toList :=
   (rfl)
 
 @[simp]
-theorem IterM.toList_toArray
-    [Monad m] [MonadAttach m] [LawfulMonad m] [LawfulMonadAttach m]
-    [Iterator α m β] [Finite α m] [IteratorCollect α m m]
+theorem IterM.toList_toArray [Monad m] [Iterator α m β] [Finite α m] [IteratorCollect α m m]
     {it : IterM (α := α) m β} :
     Array.toList <$> it.toArray = it.toList := by
   simp [IterM.toList]
 
-theorem IterM.toList_toArray_ensureTermination
-    [Monad m] [MonadAttach m] [LawfulMonad m] [LawfulMonadAttach m]
-    [Iterator α m β] [Finite α m]
+theorem IterM.toList_toArray_ensureTermination [Monad m] [Iterator α m β] [Finite α m]
     [IteratorCollect α m m] {it : IterM (α := α) m β} :
     Array.toList <$> it.ensureTermination.toArray = it.toList := by
   simp
 
 @[simp]
-theorem IterM.toArray_toList
-    [Monad m] [MonadAttach m] [LawfulMonad m] [LawfulMonadAttach m]
-    [Iterator α m β] [Finite α m]
+theorem IterM.toArray_toList [Monad m] [LawfulMonad m] [Iterator α m β] [Finite α m]
     [IteratorCollect α m m] {it : IterM (α := α) m β} :
     List.toArray <$> it.toList = it.toArray := by
   simp [IterM.toList, -toList_toArray]
 
-theorem IterM.toArray_toList_ensureTermination
-    [Monad m] [MonadAttach m] [LawfulMonad m] [LawfulMonadAttach m]
-    [Iterator α m β] [Finite α m]
+theorem IterM.toArray_toList_ensureTermination [Monad m] [LawfulMonad m] [Iterator α m β] [Finite α m]
     [IteratorCollect α m m] {it : IterM (α := α) m β} :
     List.toArray <$> it.ensureTermination.toList = it.toArray := by
   rw [toList_ensureTermination, toArray_toList]
 
-theorem IterM.toList_eq_match_step
-    [Monad m] [MonadAttach m] [LawfulMonad m] [LawfulMonadAttach m]
-    [Iterator α m β] [Finite α m]
+theorem IterM.toList_eq_match_step [Monad m] [LawfulMonad m] [Iterator α m β] [Finite α m]
     [IteratorCollect α m m] [LawfulIteratorCollect α m m] {it : IterM (α := α) m β} :
     it.toList = (do
-      match ← it.step with
+      match (← it.step).inflate.val with
       | .yield it' out => return out :: (← it'.toList)
       | .skip it' => it'.toList
       | .done => return []) := by
@@ -179,59 +144,49 @@ theorem IterM.toList_eq_match_step
   intro step
   split <;> simp
 
-theorem IterM.toList_ensureTermination_eq_match_step
-    [Monad m] [MonadAttach m] [LawfulMonad m] [LawfulMonadAttach m] [Iterator α m β]
+theorem IterM.toList_ensureTermination_eq_match_step [Monad m] [LawfulMonad m] [Iterator α m β]
     [Finite α m] [IteratorCollect α m m] [LawfulIteratorCollect α m m] {it : IterM (α := α) m β} :
     it.ensureTermination.toList = (do
-      match ← it.step with
+      match (← it.step).inflate.val with
       | .yield it' out => return out :: (← it'.toList)
       | .skip it' => it'.toList
       | .done => return []) := by
   rw [toList_ensureTermination, toList_eq_match_step]
 
 @[simp]
-theorem IterM.toListRev_ensureTermination_eq_toListRev
-    [Monad m] [MonadAttach m] [LawfulMonad m] [LawfulMonadAttach m]
-    [Iterator α m β] [Finite α m]
+theorem IterM.toListRev_ensureTermination_eq_toListRev [Monad m] [Iterator α m β] [Finite α m]
     {it : IterM (α := α) m β} :
     it.ensureTermination.toListRev = it.toListRev :=
   (rfl)
 
-private theorem IterM.toListRev.go_eq
-    [Monad m] [MonadAttach m] [LawfulMonad m] [LawfulMonadAttach m]
-    [Iterator α m β] [Finite α m]
+private theorem IterM.toListRev.go_eq [Monad m] [LawfulMonad m] [Iterator α m β] [Finite α m]
     {it : IterM (α := α) m β} {bs : List β} :
     go it bs = (do
-      match ← it.step with
+      match (← it.step).inflate.val with
       | .yield it' out => go it' (out :: bs)
       | .skip it' => go it' bs
       | .done => return bs) := by
   rw [go, WellFounded.extrinsicFix₂_eq_apply]
-  · conv => rhs; simp only [← LawfulMonadAttach.map_attach (x := it.step), bind_map_left]
-    apply bind_congr; intro step
-    cases step using PlausibleIterStep.casesOn <;> simp [go]
+  · apply bind_congr; intro step
+    cases step.inflate using PlausibleIterStep.casesOn <;> simp [go]
   · simp only [show (IterM.finitelyManySteps! = IterM.finitelyManySteps) by rfl]
     apply InvImage.wf
     exact WellFoundedRelation.wf
 
-private theorem IterM.toListRev.go.aux₁
-    [Monad m] [MonadAttach m] [LawfulMonad m] [LawfulMonadAttach m]
-    [Iterator α m β] [Finite α m]
+private theorem IterM.toListRev.go.aux₁ [Monad m] [LawfulMonad m] [Iterator α m β] [Finite α m]
     {it : IterM (α := α) m β} {b : β} {bs : List β} :
     IterM.toListRev.go it (bs ++ [b]) = (· ++ [b]) <$> IterM.toListRev.go it bs:= by
   induction it using IterM.inductSteps generalizing bs with | step it ihy ihs
   rw [go_eq, go_eq, map_eq_pure_bind, bind_assoc]
-  simp only [← LawfulMonadAttach.map_attach (x := it.step), bind_map_left]
-  apply bind_congr; intro step
-  cases step using PlausibleIterStep.casesOn
+  apply bind_congr
+  intro step
+  cases step.inflate using PlausibleIterStep.casesOn
   · simpa using ihy ‹_› (bs := _ :: bs)
   · simpa using ihs ‹_›
   · simp
 
 
-private theorem IterM.toListRev.go.aux₂
-    [Monad m] [MonadAttach m] [LawfulMonad m] [LawfulMonadAttach m]
-    [Iterator α m β] [Finite α m]
+private theorem IterM.toListRev.go.aux₂ [Monad m] [LawfulMonad m] [Iterator α m β] [Finite α m]
     {it : IterM (α := α) m β} {acc : List β} :
     IterM.toListRev.go it acc = (· ++ acc) <$> it.toListRev := by
   rw [← List.reverse_reverse (as := acc)]
@@ -240,34 +195,30 @@ private theorem IterM.toListRev.go.aux₂
   | nil => simp [toListRev]
   | cons x xs ih => simp [IterM.toListRev.go.aux₁, ih]
 
-theorem IterM.toListRev_eq_match_step
-    [Monad m] [MonadAttach m] [LawfulMonad m] [LawfulMonadAttach m]
-    [Iterator α m β] [Finite α m] {it : IterM (α := α) m β} :
+theorem IterM.toListRev_eq_match_step [Monad m] [LawfulMonad m] [Iterator α m β] [Finite α m]
+    {it : IterM (α := α) m β} :
     it.toListRev = (do
-      match ← it.step with
+      match (← it.step).inflate.val with
       | .yield it' out => return (← it'.toListRev) ++ [out]
       | .skip it' => it'.toListRev
       | .done => return []) := by
   simp [IterM.toListRev]
   rw [toListRev.go_eq]
-  simp only [← LawfulMonadAttach.map_attach (x := it.step), bind_map_left]
-  apply bind_congr; intro step
-  cases step using PlausibleIterStep.casesOn <;> simp [IterM.toListRev.go.aux₂]
+  apply bind_congr
+  intro step
+  cases step.inflate using PlausibleIterStep.casesOn <;> simp [IterM.toListRev.go.aux₂]
 
-theorem IterM.toListRev_ensureTermination_eq_match_step
-    [Monad m] [MonadAttach m] [LawfulMonad m] [LawfulMonadAttach m]
-    [Iterator α m β] [Finite α m] {it : IterM (α := α) m β} :
+theorem IterM.toListRev_ensureTermination_eq_match_step [Monad m] [LawfulMonad m] [Iterator α m β]
+    [Finite α m] {it : IterM (α := α) m β} :
     it.ensureTermination.toListRev = (do
-      match ← it.step with
+      match (← it.step).inflate.val with
       | .yield it' out => return (← it'.toListRev) ++ [out]
       | .skip it' => it'.toListRev
       | .done => return []) := by
   rw [toListRev_ensureTermination_eq_toListRev, toListRev_eq_match_step]
 
 @[simp]
-theorem IterM.reverse_toListRev
-    [Monad m] [MonadAttach m] [LawfulMonad m] [LawfulMonadAttach m]
-    [Iterator α m β] [Finite α m]
+theorem IterM.reverse_toListRev [Monad m] [LawfulMonad m] [Iterator α m β] [Finite α m]
     [IteratorCollect α m m] [LawfulIteratorCollect α m m]
     {it : IterM (α := α) m β} :
     List.reverse <$> it.toListRev = it.toList := by
@@ -275,48 +226,38 @@ theorem IterM.reverse_toListRev
   induction it using IterM.inductSteps
   rename_i it ihy ihs
   rw [toListRev_eq_match_step, toList_eq_match_step, map_eq_pure_bind, bind_assoc]
-  simp only [← LawfulMonadAttach.map_attach (x := it.step), bind_map_left]
-  apply bind_congr; intro step
-  cases step using PlausibleIterStep.casesOn
-  · simp [ihy ‹_›]
-  · simp [ihs ‹_›]
-  · simp
+  apply bind_congr
+  intro step
+  cases step.inflate using PlausibleIterStep.casesOn <;> simp (discharger := assumption) [ihy, ihs]
 
 @[simp]
-theorem IterM.reverse_toListRev_ensureTermination
-    [Monad m] [MonadAttach m] [LawfulMonad m] [LawfulMonadAttach m]
-    [Iterator α m β] [Finite α m] [IteratorCollect α m m] [LawfulIteratorCollect α m m]
+theorem IterM.reverse_toListRev_ensureTermination [Monad m] [LawfulMonad m] [Iterator α m β]
+    [Finite α m] [IteratorCollect α m m] [LawfulIteratorCollect α m m]
     {it : IterM (α := α) m β} :
     List.reverse <$> it.ensureTermination.toListRev = it.toList := by
   rw [toListRev_ensureTermination_eq_toListRev, reverse_toListRev]
 
-theorem IterM.toListRev_eq
-    [Monad m] [MonadAttach m] [LawfulMonad m] [LawfulMonadAttach m]
-    [Iterator α m β] [Finite α m]
+theorem IterM.toListRev_eq [Monad m] [LawfulMonad m] [Iterator α m β] [Finite α m]
     [IteratorCollect α m m] [LawfulIteratorCollect α m m]
     {it : IterM (α := α) m β} :
     it.toListRev = List.reverse <$> it.toList := by
   simp [← IterM.reverse_toListRev]
 
-theorem IterM.toListRev_ensureTermination
-    [Monad m] [MonadAttach m] [LawfulMonad m] [LawfulMonadAttach m]
-    [Iterator α m β] [Finite α m]
+theorem IterM.toListRev_ensureTermination [Monad m] [LawfulMonad m] [Iterator α m β] [Finite α m]
     [IteratorCollect α m m] [LawfulIteratorCollect α m m]
     {it : IterM (α := α) m β} :
     it.ensureTermination.toListRev = List.reverse <$> it.toList := by
   simp [← IterM.reverse_toListRev]
 
 theorem LawfulIteratorCollect.toArray_eq {α β : Type w} {m : Type w → Type w'}
-    [Monad m] [MonadAttach m] [LawfulMonad m] [LawfulMonadAttach m]
-    [Iterator α m β] [Finite α m] [IteratorCollect α m m]
+    [Monad m] [Iterator α m β] [Finite α m] [IteratorCollect α m m]
     [hl : LawfulIteratorCollect α m m]
     {it : IterM (α := α) m β} :
     it.toArray = (letI : IteratorCollect α m m := .defaultImplementation; it.toArray) := by
   simp [IterM.toArray, toArrayMapped_eq, IteratorCollect.defaultImplementation]
 
 theorem LawfulIteratorCollect.toList_eq {α β : Type w} {m : Type w → Type w'}
-    [Monad m] [MonadAttach m] [LawfulMonad m] [LawfulMonadAttach m]
-    [Iterator α m β] [Finite α m] [IteratorCollect α m m]
+    [Monad m] [Iterator α m β] [Finite α m] [IteratorCollect α m m]
     [hl : LawfulIteratorCollect α m m]
     {it : IterM (α := α) m β} :
     it.toList = (letI : IteratorCollect α m m := .defaultImplementation; it.toList) := by
