src/Init/Data/Iterators/Lemmas/Consumers/Monadic/Loop.lean
@@ -15,32 +15,31 @@ public section
 namespace Std.Iterators
 
 theorem IterM.DefaultConsumers.forIn'_eq_match_step {α β : Type w} {m : Type w → Type w'}
-    [Iterator α m β] {n : Type x → Type x'} [MonadAttach m]
-    [Monad n] [MonadAttach n] [LawfulMonad n] [LawfulMonadAttach n]
+    [Iterator α m β] {n : Type x → Type x'} [Monad n] [LawfulMonad n]
     {lift : ∀ γ δ, (γ → n δ) → m γ → n δ} {γ : Type x}
     {it : IterM (α := α) m β} {init : γ}
     {P hP}
-    {f : (b : β) → P b → (c : γ) → n (ForInStep γ)}
-    (wf : IteratorLoop.WellFounded α m (fun b hb c => MonadAttach.CanReturn (f b hb c))) :
-    IterM.DefaultConsumers.forIn' lift γ it init P hP f =
-      (lift _ _ · (MonadAttach.attach it.step)) (fun s =>
-          match s with
-          | ⟨.yield it' out, h⟩ => do
+    (PlausibleForInStep : β → γ → ForInStep γ → Prop)
+    {f : (b : β) → P b → (c : γ) → n (Subtype (PlausibleForInStep b c))}
+    (wf : IteratorLoop.WellFounded α m PlausibleForInStep) :
+    IterM.DefaultConsumers.forIn' lift γ PlausibleForInStep it init P hP f =
+      (lift _ _ · it.step) (fun s =>
+          match s.inflate with
+          | .yield it' out h => do
             match ← f out (hP _ <| .direct ⟨_, h⟩) init with
-            | .yield c =>
-              IterM.DefaultConsumers.forIn' lift _ it' c P
+            | ⟨.yield c, _⟩ =>
+              IterM.DefaultConsumers.forIn' lift _ PlausibleForInStep it' c P
                 (fun _ h' => hP _ <| .indirect ⟨_, rfl, h⟩ h') f
-            | .done c => return c
-          | ⟨.skip it', h⟩ =>
-            IterM.DefaultConsumers.forIn' lift _ it' init P
+            | ⟨.done c, _⟩ => return c
+          | .skip it' h =>
+            IterM.DefaultConsumers.forIn' lift _ PlausibleForInStep it' init P
               (fun _ h' => hP _ <| .indirect ⟨_, rfl, h⟩ h') f
-          | ⟨.done, _⟩ => return init) := by
+          | .done _ => return init) := by
   haveI : Nonempty γ := ⟨init⟩
   rw [forIn', WellFounded.extrinsicFix₃_eq_apply]
   · congr; ext step
-    cases step using PlausibleIterStep.casesOn
+    cases step.inflate using PlausibleIterStep.casesOn
     · simp only
-      conv => rhs; simp only [← LawfulMonadAttach.map_attach (x := f _ _ _), bind_map_left]
       apply bind_congr; intro step
       split <;> simp [forIn']
     · simp [forIn']
@@ -50,25 +49,24 @@ theorem IterM.DefaultConsumers.forIn'_eq_match_step {α β : Type w} {m : Type w
 
 theorem IterM.DefaultConsumers.forIn'_eq_wf {m : Type w → Type w'} {α : Type w} {β : Type w}
     [Iterator α m β]
-    {n : Type x → Type x'}
-    [MonadAttach m]
-    [Monad n] [MonadAttach n] [LawfulMonad n]
+    {n : Type x → Type x'} [Monad n] [LawfulMonad n]
     {lift : ∀ γ δ, (γ → n δ) → m γ → n δ} {γ : Type x}
+    (Pl : β → γ → ForInStep γ → Prop)
+    (wf : IteratorLoop.WellFounded α m Pl)
     {it : IterM (α := α) m β} {init : γ}
     {P : β → Prop} {hP : ∀ b, it.IsPlausibleIndirectOutput b → P b}
-    (f : (b : β) → P b → (c : γ) → n (ForInStep γ))
-    (wf : IteratorLoop.WellFounded α m (MonadAttach.CanReturn <| f · · ·)) :
-    forIn' lift γ it init P hP f =
-      forIn'.wf lift γ it init P hP f wf := by
+    (f : (b : β) → P b → (c : γ) → n (Subtype (Pl b c))) :
+    forIn' lift γ Pl it init P hP f =
+      forIn'.wf lift γ Pl wf it init P hP f := by
   haveI : Nonempty γ := ⟨init⟩
   rw [forIn', WellFounded.extrinsicFix₃_eq_fix]; rotate_left
   · apply InvImage.wf
     exact wf
-  · fun_induction forIn'.wf lift γ it init P hP f wf
+  · fun_induction forIn'.wf lift γ Pl wf it init P hP f
     rename_i ihy ihs
     rw [WellFounded.fix_eq]
     congr 1; ext step
-    cases step using PlausibleIterStep.casesOn
+    cases step.inflate using PlausibleIterStep.casesOn
     · apply bind_congr; intro forInStep
       match forInStep with
       | ⟨.yield c, h⟩ => simp (discharger := assumption) [ihy]
@@ -77,50 +75,41 @@ theorem IterM.DefaultConsumers.forIn'_eq_wf {m : Type w → Type w'} {α : Type 
     · simp
 
 theorem IterM.DefaultConsumers.forIn'_eq_wf_of_finite {m : Type w → Type w'} {α : Type w}
-    {β : Type w} {n : Type x → Type x'}
-    [MonadAttach m]
-    [Monad n] [MonadAttach n] [LawfulMonad n]
-    [Iterator α m β] [Finite α m]
+    {β : Type w} [Iterator α m β] [Finite α m]
+    {n : Type x → Type x'} [Monad n] [LawfulMonad n]
     {lift : ∀ γ δ, (γ → n δ) → m γ → n δ} {γ : Type x}
     {it : IterM (α := α) m β} {init : γ}
     {P : β → Prop} {hP : ∀ b, it.IsPlausibleIndirectOutput b → P b}
-    (f : (b : β) → P b → (c : γ) → n (ForInStep γ)) :
-    forIn' lift γ it init P hP f =
-      forIn'.wf lift γ it init P hP f IteratorLoop.wellFounded_of_finite := by
+    (f : (b : β) → P b → (c : γ) → n (Subtype (fun _ => True))) :
+    forIn' lift γ (fun _ _ _ => True) it init P hP f =
+      forIn'.wf lift γ (fun _ _ _ => True) IteratorLoop.wellFounded_of_finite it init P hP f := by
   apply forIn'_eq_wf
 
-theorem IterM.forIn'_eq {α β : Type w} {m : Type w → Type w'} {n : Type w → Type w''}
-    [Monad m] [MonadAttach m]
-    [Monad n] [MonadAttach n] [LawfulMonad n]
-    [Iterator α m β] [Finite α m]
-    [IteratorLoop α m n]
+theorem IterM.forIn'_eq {α β : Type w} {m : Type w → Type w'} [Iterator α m β] [Finite α m]
+    {n : Type w → Type w''} [Monad m] [Monad n] [LawfulMonad n] [IteratorLoop α m n]
     [hl : LawfulIteratorLoop α m n]
     [MonadLiftT m n] [LawfulMonadLiftT m n] {γ : Type w} {it : IterM (α := α) m β} {init : γ}
     {f : (b : β) → it.IsPlausibleIndirectOutput b → γ → n (ForInStep γ)} :
     letI : ForIn' n (IterM (α := α) m β) β _ := IterM.instForIn'
     ForIn'.forIn' (α := β) (m := n) it init f = IterM.DefaultConsumers.forIn' (n := n)
-        (fun _ _ f x => monadLift x >>= f) γ it init _ (fun _ => id) f := by
+        (fun _ _ f x => monadLift x >>= f) γ (fun _ _ _ => True) it init _ (fun _ => id) (return ⟨← f · · ·, trivial⟩) := by
   simp only [instForIn', ForIn'.forIn', IteratorLoop.finiteForIn']
   have : f = (Subtype.val <$> (⟨·, trivial⟩) <$> f · · ·) := by simp
   rw [this, hl.lawful (fun _ _ f x => monadLift x >>= f) (wf := IteratorLoop.wellFounded_of_finite)]
   simp [IteratorLoop.defaultImplementation]
 
-theorem IterM.forIn_eq {α β : Type w} {m : Type w → Type w'} {n : Type w → Type w''}
-    [Monad m] [MonadAttach m]
-    [Monad n] [MonadAttach n] [LawfulMonad n]
-    [Iterator α m β] [Finite α m]
-    [IteratorLoop α m n]
+theorem IterM.forIn_eq {α β : Type w} {m : Type w → Type w'} [Iterator α m β] [Finite α m]
+    {n : Type w → Type w''} [Monad m] [Monad n] [LawfulMonad n] [IteratorLoop α m n]
     [hl : LawfulIteratorLoop α m n]
     [MonadLiftT m n] [LawfulMonadLiftT m n] {γ : Type w} {it : IterM (α := α) m β} {init : γ}
     {f : β → γ → n (ForInStep γ)} :
     ForIn.forIn it init f = IterM.DefaultConsumers.forIn' (n := n)
-        (fun _ _ f x => monadLift x >>= f) γ it init _ (fun _ => id)
-        (fun out _ acc => f out acc) := by
+        (fun _ _ f x => monadLift x >>= f) γ (fun _ _ _ => True) it init _ (fun _ => id)
+        (fun out _ acc => return ⟨← f out acc, trivial⟩) := by
   simp only [ForIn.forIn, forIn'_eq]
 
 @[congr] theorem IterM.forIn'_congr {α β : Type w} {m : Type w → Type w'}
-    {n : Type w → Type w''}
-    [Monad m] [MonadAttach m] [Monad n] [MonadAttach n]
+    {n : Type w → Type w''} [Monad n] [Monad m]
     [Iterator α m β] [IteratorLoop α m n] [MonadLiftT m n]
     {ita itb : IterM (α := α) m β} (w : ita = itb)
     {b b' : γ} (hb : b = b')
@@ -135,8 +124,7 @@ theorem IterM.forIn_eq {α β : Type w} {m : Type w → Type w'} {n : Type w →
   rfl
 
 @[congr] theorem IterM.forIn_congr {α β : Type w} {m : Type w → Type w'}
-    {n : Type w → Type w''}
-    [Monad m] [MonadAttach m] [Monad n] [MonadAttach n]
+    {n : Type w → Type w''} [Monad n] [Monad m]
     [Iterator α m β] [IteratorLoop α m n] [MonadLiftT m n]
     {ita itb : IterM (α := α) m β} (w : ita = itb)
     {b b' : γ} (hb : b = b')
@@ -149,223 +137,194 @@ theorem IterM.forIn_eq {α β : Type w} {m : Type w → Type w'} {n : Type w →
   rw [← h]
 
 theorem IterM.DefaultConsumers.forIn'_eq_forIn' {m : Type w → Type w'} {α : Type w} {β : Type w}
-    [Iterator α m β] {n : Type x → Type x'}
-    [MonadAttach m]
-    [Monad n] [MonadAttach n] [LawfulMonad n] [LawfulMonadAttach n]
+    [Iterator α m β]
+    {n : Type x → Type x'} [Monad n] [LawfulMonad n]
     {lift : ∀ γ δ, (γ → n δ) → m γ → n δ} {γ : Type x}
     {it : IterM (α := α) m β} {init : γ}
     {P : β → Prop} {hP : ∀ b, it.IsPlausibleIndirectOutput b → P b}
     {Q : β → Prop} {hQ : ∀ b, it.IsPlausibleIndirectOutput b → Q b}
-    {f : (b : β) → P b → (c : γ) → n (ForInStep γ)}
-    {g : (b : β) → Q b → (c : γ) → n (ForInStep γ)}
-    (wf : IteratorLoop.WellFounded α m (MonadAttach.CanReturn <| f · · ·))
-    (wf' : IteratorLoop.WellFounded α m (MonadAttach.CanReturn <| g · · ·))
+    (Pl : β → γ → ForInStep γ → Prop)
+    {f : (b : β) → P b → (c : γ) → n (Subtype (Pl b c))}
+    {g : (b : β) → Q b → (c : γ) → n (Subtype (Pl b c))}
+    (wf : IteratorLoop.WellFounded α m Pl)
     (hfg : ∀ b c, (hPb : P b) → (hQb : Q b) → f b hPb c = g b hQb c) :
-    IterM.DefaultConsumers.forIn' lift γ it init P hP f =
-      IterM.DefaultConsumers.forIn' lift γ it init Q hQ g := by
-  rw [forIn'_eq_match_step wf, forIn'_eq_match_step wf']
-  simp only
+    IterM.DefaultConsumers.forIn' lift γ Pl it init P hP f =
+      IterM.DefaultConsumers.forIn' lift γ Pl it init Q hQ g := by
+  rw [forIn'_eq_match_step Pl wf, forIn'_eq_match_step Pl wf]
   congr; ext step
   split
-  · simp only [← LawfulMonadAttach.map_attach (x := f _ _ _),
-      ← LawfulMonadAttach.map_attach (x  := g _ _ _), bind_map_left]
-    rw [← hfg (hPb := hP _ (.direct ⟨_, ‹_›⟩))]
-    apply bind_congr; intro a
-    match a with
-    | ⟨.yield _, _⟩ =>
-      simp only
-      apply IterM.DefaultConsumers.forIn'_eq_forIn' <;> assumption
-    | ⟨.done _, _⟩ => simp
+  · congr
+    · apply hfg
+    · ext forInStep
+      match forInStep with
+      | ⟨.yield _, h⟩ => apply IterM.DefaultConsumers.forIn'_eq_forIn' <;> assumption
+      | ⟨.done _, h⟩ => rfl
   · apply IterM.DefaultConsumers.forIn'_eq_forIn' <;> assumption
   · rfl
 termination_by IteratorLoop.WithWF.mk it init (hwf := wf)
 decreasing_by
-  · exact Or.inl ⟨_, hP _ (.direct ⟨_, ‹_›⟩), ‹_›, ‹_›⟩
+  · exact Or.inl ⟨_, ‹_›, ‹_›⟩
   · exact Or.inr ⟨‹_›, rfl⟩
 
-theorem IterM.forIn'_eq_match_step {α β : Type w} {m : Type w → Type w'} {n : Type w → Type w''}
-    [Monad m] [MonadAttach m]
-    [Monad n] [MonadAttach n] [LawfulMonad n] [LawfulMonadAttach n]
-    [Iterator α m β] [Finite α m]
+theorem IterM.forIn'_eq_match_step {α β : Type w} {m : Type w → Type w'} [Iterator α m β]
+    [Finite α m] {n : Type w → Type w''} [Monad m] [Monad n] [LawfulMonad n]
     [IteratorLoop α m n] [LawfulIteratorLoop α m n]
     [MonadLiftT m n] [LawfulMonadLiftT m n] {γ : Type w} {it : IterM (α := α) m β} {init : γ}
     {f : (out : β) → _ → γ → n (ForInStep γ)} :
     letI : ForIn' n (IterM (α := α) m β) β _ := IterM.instForIn'
     ForIn'.forIn' it init f = (do
-      match ← MonadAttach.attach it.step with
-      | ⟨.yield it' out, h⟩ =>
+      match (← it.step).inflate with
+      | .yield it' out h =>
         match ← f out (.direct ⟨_, h⟩) init with
         | .yield c =>
           ForIn'.forIn' it' c
             fun out h'' acc => f out (.indirect ⟨_, rfl, h⟩ h'') acc
         | .done c => return c
-      | ⟨.skip it', h⟩ =>
+      | .skip it' h =>
         ForIn'.forIn' it' init
           fun out h' acc => f out (.indirect ⟨_, rfl, h⟩ h') acc
-      | ⟨.done, _⟩ => return init) := by
+      | .done _ => return init) := by
   rw [IterM.forIn'_eq, DefaultConsumers.forIn'_eq_match_step]
   · apply bind_congr; intro step
-    cases step using PlausibleIterStep.casesOn
-    · apply bind_congr; intro forInStep
+    cases step.inflate using PlausibleIterStep.casesOn
+    · simp only [bind_assoc]
+      apply bind_congr
+      intro forInStep
       cases forInStep
       · simp
-      · simp only [forIn'_eq]
-        exact DefaultConsumers.forIn'_eq_forIn' (α := α) (m := m) (n := n) IteratorLoop.wellFounded_of_finite
+      · simp only [forIn'_eq, pure_bind]
+        exact DefaultConsumers.forIn'_eq_forIn' (α := α) (m := m) (n := n) _
           IteratorLoop.wellFounded_of_finite (by simp)
     · simp only [forIn'_eq]
-      exact DefaultConsumers.forIn'_eq_forIn' (α := α) (m := m) (n := n) IteratorLoop.wellFounded_of_finite
+      exact DefaultConsumers.forIn'_eq_forIn' (α := α) (m := m) (n := n) _
           IteratorLoop.wellFounded_of_finite (by simp)
     · simp
   · exact IteratorLoop.wellFounded_of_finite
 
-theorem IterM.forIn_eq_match_step {α β : Type w} {m : Type w → Type w'} {n : Type w → Type w''}
-    [Monad m] [MonadAttach m] [LawfulMonad m] [LawfulMonadAttach m]
-    [Monad n] [MonadAttach n] [LawfulMonad n] [LawfulMonadAttach n]
-    [Iterator α m β] [Finite α m]
+theorem IterM.forIn_eq_match_step {α β : Type w} {m : Type w → Type w'} [Iterator α m β]
+    [Finite α m] {n : Type w → Type w''} [Monad m] [Monad n] [LawfulMonad n]
     [IteratorLoop α m n] [LawfulIteratorLoop α m n]
     [MonadLiftT m n] [LawfulMonadLiftT m n] {γ : Type w} {it : IterM (α := α) m β} {init : γ}
     {f : β → γ → n (ForInStep γ)} :
     ForIn.forIn it init f = (do
-      match ← it.step with
-      | .yield it' out =>
+      match (← it.step).inflate with
+      | .yield it' out _ =>
         match ← f out init with
         | .yield c => ForIn.forIn it' c f
         | .done c => return c
-      | .skip it' => ForIn.forIn it' init f
-      | .done => return init) := by
+      | .skip it' _ => ForIn.forIn it' init f
+      | .done _ => return init) := by
   simp only [forIn]
-  rw [forIn'_eq_match_step]
-  conv => rhs; simp only [← LawfulMonadAttach.map_attach (x := it.step), liftM_map, bind_map_left]
-  apply bind_congr; intro step
-  cases step using PlausibleIterStep.casesOn <;> simp
+  exact forIn'_eq_match_step
 
-theorem IterM.forM_eq_forIn {α β : Type w} {m : Type w → Type w'} {n : Type w → Type w''}
-    [Monad m] [MonadAttach m]
-    [Monad n] [MonadAttach n]
-    [Iterator α m β] [IteratorLoop α m n]
+theorem IterM.forM_eq_forIn {α β : Type w} {m : Type w → Type w'} [Iterator α m β]
+    [Finite α m] {n : Type w → Type w''} [Monad m] [Monad n] [LawfulMonad n]
+    [IteratorLoop α m n] [LawfulIteratorLoop α m n]
     [MonadLiftT m n] {it : IterM (α := α) m β}
     {f : β → n PUnit} :
     ForM.forM it f = ForIn.forIn it PUnit.unit (fun out _ => do f out; return .yield .unit) :=
   rfl
 
-theorem IterM.forM_eq_match_step {α β : Type w} {m : Type w → Type w'} {n : Type w → Type w''}
-    [Monad m] [MonadAttach m] [LawfulMonad m] [LawfulMonadAttach m]
-    [Monad n] [MonadAttach n] [LawfulMonad n] [LawfulMonadAttach n]
-    [Iterator α m β] [Finite α m]
+theorem IterM.forM_eq_match_step {α β : Type w} {m : Type w → Type w'} [Iterator α m β]
+    [Finite α m] {n : Type w → Type w''} [Monad m] [Monad n] [LawfulMonad n]
     [IteratorLoop α m n] [LawfulIteratorLoop α m n]
     [MonadLiftT m n] [LawfulMonadLiftT m n] {it : IterM (α := α) m β}
     {f : β → n PUnit} :
     ForM.forM it f = (do
-      match ← it.step with
-      | .yield it' out =>
+      match (← it.step).inflate with
+      | .yield it' out _ =>
         f out
         ForM.forM it' f
-      | .skip it' => ForM.forM it' f
-      | .done => return) := by
+      | .skip it' _ => ForM.forM it' f
+      | .done _ => return) := by
   rw [forM_eq_forIn, forIn_eq_match_step]
-  apply bind_congr; intro step
-  cases step <;> simp [forM_eq_forIn]
+  apply bind_congr
+  intro step
+  cases step.inflate using PlausibleIterStep.casesOn <;> simp [forM_eq_forIn]
 
-theorem IterM.foldM_eq_forIn {α β γ : Type w} {m : Type w → Type w'} {n : Type w → Type w''}
-    [MonadAttach m]
-    [Monad n] [MonadAttach n]
-    [Iterator α m β] [IteratorLoop α m n] [MonadLiftT m n]
-    {f : γ → β → n γ} {init : γ} {it : IterM (α := α) m β} :
+theorem IterM.foldM_eq_forIn {α β γ : Type w} {m : Type w → Type w'} [Iterator α m β] [Finite α m]
+    {n : Type w → Type w''} [Monad n] [IteratorLoop α m n] [MonadLiftT m n] {f : γ → β → n γ}
+    {init : γ} {it : IterM (α := α) m β} :
     it.foldM (init := init) f = ForIn.forIn it init (fun x acc => ForInStep.yield <$> f acc x) :=
   (rfl)
 
-theorem IterM.forIn_yield_eq_foldM {α β γ δ : Type w} {m : Type w → Type w'} {n : Type w → Type w''}
-    [Monad m] [MonadAttach m]
-    [Monad n] [MonadAttach n] [LawfulMonad n]
-    [Iterator α m β] [Finite α m] [IteratorLoop α m n]
+theorem IterM.forIn_yield_eq_foldM {α β γ δ : Type w} {m : Type w → Type w'} [Iterator α m β]
+    [Finite α m] {n : Type w → Type w''} [Monad m] [Monad n] [LawfulMonad n] [IteratorLoop α m n]
     [LawfulIteratorLoop α m n] [MonadLiftT m n] {f : β → γ → n δ} {g : β → γ → δ → γ} {init : γ}
     {it : IterM (α := α) m β} :
     ForIn.forIn it init (fun c b => (fun d => .yield (g c b d)) <$> f c b) =
       it.foldM (fun b c => g c b <$> f c b) init := by
   simp [IterM.foldM_eq_forIn]
 
-theorem IterM.foldM_eq_match_step {α β γ : Type w} {m : Type w → Type w'} {n : Type w → Type w''}
-    [Monad m] [MonadAttach m] [LawfulMonad m] [LawfulMonadAttach m]
-    [Monad n] [MonadAttach n] [LawfulMonad n] [LawfulMonadAttach n]
-    [Iterator α m β] [Finite α m]
-    [IteratorLoop α m n]
+theorem IterM.foldM_eq_match_step {α β γ : Type w} {m : Type w → Type w'} [Iterator α m β] [Finite α m]
+    {n : Type w → Type w''} [Monad m] [Monad n] [LawfulMonad n] [IteratorLoop α m n]
     [LawfulIteratorLoop α m n] [MonadLiftT m n] [LawfulMonadLiftT m n]
     {f : γ → β → n γ} {init : γ} {it : IterM (α := α) m β} :
     it.foldM (init := init) f = (do
-      match ← it.step with
-      | .yield it' out => it'.foldM (init := ← f init out) f
-      | .skip it' => it'.foldM (init := init) f
-      | .done => return init) := by
+      match (← it.step).inflate with
+      | .yield it' out _ => it'.foldM (init := ← f init out) f
+      | .skip it' _ => it'.foldM (init := init) f
+      | .done _ => return init) := by
   rw [IterM.foldM_eq_forIn, IterM.forIn_eq_match_step]
-  apply bind_congr; intro step
-  cases step <;> simp [foldM_eq_forIn]
+  apply bind_congr
+  intro step
+  cases step.inflate using PlausibleIterStep.casesOn <;> simp [foldM_eq_forIn]
 
-theorem IterM.fold_eq_forIn {α β γ : Type w} {m : Type w → Type w'}
-    [Monad m] [MonadAttach m]
-    [Iterator α m β]
+theorem IterM.fold_eq_forIn {α β γ : Type w} {m : Type w → Type w'} [Iterator α m β]
+    [Finite α m] [Monad m]
     [IteratorLoop α m m] {f : γ → β → γ} {init : γ} {it : IterM (α := α) m β} :
     it.fold (init := init) f =
       ForIn.forIn (m := m) it init (fun x acc => pure (ForInStep.yield (f acc x))) := by
   rfl
 
-theorem IterM.fold_eq_foldM {α β γ : Type w} {m : Type w → Type w'}
-    [Monad m] [MonadAttach m] [LawfulMonad m]
-    [Iterator α m β]
-    [Finite α m] [IteratorLoop α m m] {f : γ → β → γ} {init : γ}
+theorem IterM.fold_eq_foldM {α β γ : Type w} {m : Type w → Type w'} [Iterator α m β]
+    [Finite α m] [Monad m] [LawfulMonad m] [IteratorLoop α m m] {f : γ → β → γ} {init : γ}
     {it : IterM (α := α) m β} :
     it.fold (init := init) f = it.foldM (init := init) (pure <| f · ·) := by
   simp [foldM_eq_forIn, fold_eq_forIn]
 
 @[simp]
-theorem IterM.forIn_pure_yield_eq_fold {α β γ : Type w} {m : Type w → Type w'}
-    [Monad m] [MonadAttach m] [LawfulMonad m]
-    [Iterator α m β] [Finite α m] [IteratorLoop α m m]
+theorem IterM.forIn_pure_yield_eq_fold {α β γ : Type w} {m : Type w → Type w'} [Iterator α m β]
+    [Finite α m] [Monad m] [LawfulMonad m] [IteratorLoop α m m]
     [LawfulIteratorLoop α m m] {f : β → γ → γ} {init : γ}
     {it : IterM (α := α) m β} :
     ForIn.forIn it init (fun c b => pure (.yield (f c b))) =
       it.fold (fun b c => f c b) init := by
   simp [IterM.fold_eq_forIn]
 
-theorem IterM.fold_eq_match_step {α β γ : Type w} {m : Type w → Type w'}
-    [Monad m] [MonadAttach m] [LawfulMonad m] [LawfulMonadAttach m]
-    [Iterator α m β] [Finite α m]
-    [IteratorLoop α m m] [LawfulIteratorLoop α m m]
+theorem IterM.fold_eq_match_step {α β γ : Type w} {m : Type w → Type w'} [Iterator α m β] [Finite α m]
+    [Monad m] [LawfulMonad m] [IteratorLoop α m m] [LawfulIteratorLoop α m m]
     {f : γ → β → γ} {init : γ} {it : IterM (α := α) m β} :
     it.fold (init := init) f = (do
-      match ← it.step with
-      | .yield it' out => it'.fold (init := f init out) f
-      | .skip it' => it'.fold (init := init) f
-      | .done => return init) := by
+      match (← it.step).inflate with
+      | .yield it' out _ => it'.fold (init := f init out) f
+      | .skip it' _ => it'.fold (init := init) f
+      | .done _ => return init) := by
   rw [fold_eq_foldM, foldM_eq_match_step]
   simp only [fold_eq_foldM]
-  simp only [← LawfulMonadAttach.map_attach (x := it.step), liftM_map, bind_map_left]
-  apply bind_congr; intro step
-  cases step using PlausibleIterStep.casesOn <;> simp
+  apply bind_congr
+  intro step
+  cases step.inflate using PlausibleIterStep.casesOn <;> simp
 
 -- The argument `f : γ₁ → γ₂` is intentionally explicit, as it is sometimes not found by unification.
-theorem IterM.fold_hom {m : Type w → Type w'}
-    [Monad m] [MonadAttach m] [LawfulMonad m] [LawfulMonadAttach m]
-    [Iterator α m β] [Finite α m]
-    [IteratorLoop α m m] [LawfulIteratorLoop α m m]
+theorem IterM.fold_hom {m : Type w → Type w'} [Iterator α m β] [Finite α m]
+    [Monad m] [LawfulMonad m] [IteratorLoop α m m] [LawfulIteratorLoop α m m]
     {it : IterM (α := α) m β}
     (f : γ₁ → γ₂) {g₁ : γ₁ → β → γ₁} {g₂ : γ₂ → β → γ₂} {init : γ₁}
     (H : ∀ x y, g₂ (f x) y = f (g₁ x y)) :
     it.fold g₂ (f init) = f <$> (it.fold g₁ init) := by
   induction it using IterM.inductSteps generalizing init with | step it ihy ihs =>
   rw [fold_eq_match_step, fold_eq_match_step, map_eq_pure_bind, bind_assoc]
-  simp only [← LawfulMonadAttach.map_attach (x := it.step), bind_map_left,
-    bind_pure_comp]
-  apply bind_congr; intro step
-  cases step using PlausibleIterStep.casesOn
-  · simp only
-    rw [H, ihy ‹_›]
-  · simp only
-    rw [ihs ‹_›]
+  apply bind_congr
+  intro step
+  rw [bind_pure_comp]
+  split
+  · rw [H, ihy ‹_›]
+  · rw [ihs ‹_›]
   · simp
 
-theorem IterM.toList_eq_fold {α β : Type w} {m : Type w → Type w'}
-    [Monad m] [MonadAttach m] [LawfulMonad m] [LawfulMonadAttach m]
-    [Iterator α m β] [Finite α m] [IteratorLoop α m m] [LawfulIteratorLoop α m m]
+theorem IterM.toList_eq_fold {α β : Type w} {m : Type w → Type w'} [Iterator α m β]
+    [Finite α m] [Monad m] [LawfulMonad m] [IteratorLoop α m m] [LawfulIteratorLoop α m m]
     [IteratorCollect α m m] [LawfulIteratorCollect α m m]
     {it : IterM (α := α) m β} :
     it.toList = it.fold (init := []) (fun l out => l ++ [out]) := by
@@ -377,9 +336,9 @@ theorem IterM.toList_eq_fold {α β : Type w} {m : Type w → Type w'}
   intro l'
   rw [IterM.toList_eq_match_step, IterM.fold_eq_match_step]
   simp only [map_eq_pure_bind, bind_assoc]
-  simp only [← LawfulMonadAttach.map_attach (x := it.step), bind_map_left]
-  apply bind_congr; intro step
-  cases step using PlausibleIterStep.casesOn
+  apply bind_congr
+  intro step
+  cases step.inflate using PlausibleIterStep.casesOn
   · rename_i it' out h
     specialize ihy h (l' ++ [out])
     simpa using ihy
@@ -387,9 +346,8 @@ theorem IterM.toList_eq_fold {α β : Type w} {m : Type w → Type w'}
     simp [ihs h]
   · simp
 
-theorem IterM.toArray_eq_fold {α β : Type w} {m : Type w → Type w'}
-    [Monad m] [MonadAttach m] [LawfulMonad m]  [LawfulMonadAttach m]
-    [Iterator α m β] [Finite α m] [IteratorLoop α m m] [LawfulIteratorLoop α m m]
+theorem IterM.toArray_eq_fold {α β : Type w} {m : Type w → Type w'} [Iterator α m β]
+    [Finite α m] [Monad m] [LawfulMonad m] [IteratorLoop α m m] [LawfulIteratorLoop α m m]
     [IteratorCollect α m m] [LawfulIteratorCollect α m m]
     {it : IterM (α := α) m β} :
     it.toArray = it.fold (init := #[]) (fun xs out => xs.push out) := by
@@ -397,94 +355,80 @@ theorem IterM.toArray_eq_fold {α β : Type w} {m : Type w → Type w'}
   rw [← fold_hom]
   simp
 
-theorem IterM.drain_eq_fold {α β : Type w} {m : Type w → Type w'}
-    [Monad m] [MonadAttach m]
-    [Iterator α m β]
-    [IteratorLoop α m m] {it : IterM (α := α) m β} :
+theorem IterM.drain_eq_fold {α β : Type w} {m : Type w → Type w'} [Iterator α m β] [Finite α m]
+    [Monad m] [IteratorLoop α m m] {it : IterM (α := α) m β} :
     it.drain = it.fold (init := PUnit.unit) (fun _ _ => .unit) :=
   (rfl)
 
-theorem IterM.drain_eq_foldM {α β : Type w} {m : Type w → Type w'}
-    [Monad m] [MonadAttach m] [LawfulMonad m]
-    [Iterator α m β] [Finite α m]
-    [IteratorLoop α m m] {it : IterM (α := α) m β} :
+theorem IterM.drain_eq_foldM {α β : Type w} {m : Type w → Type w'} [Iterator α m β] [Finite α m]
+    [Monad m] [LawfulMonad m] [IteratorLoop α m m] {it : IterM (α := α) m β} :
     it.drain = it.foldM (init := PUnit.unit) (fun _ _ => pure .unit) := by
   simp [IterM.drain_eq_fold, IterM.fold_eq_foldM]
 
-theorem IterM.drain_eq_forIn {α β : Type w} {m : Type w → Type w'}
-    [Monad m] [MonadAttach m]
-    [Iterator α m β] [Finite α m]
-    [IteratorLoop α m m] {it : IterM (α := α) m β} :
+theorem IterM.drain_eq_forIn {α β : Type w} {m : Type w → Type w'}  [Iterator α m β] [Finite α m]
+    [Monad m] [IteratorLoop α m m] {it : IterM (α := α) m β} :
     it.drain = ForIn.forIn (m := m) it PUnit.unit (fun _ _ => pure (ForInStep.yield .unit)) := by
   simp [IterM.drain_eq_fold, IterM.fold_eq_forIn]
 
-theorem IterM.drain_eq_match_step {α β : Type w} {m : Type w → Type w'}
-    [Monad m] [MonadAttach m] [LawfulMonad m] [LawfulMonadAttach m]
-    [Iterator α m β] [Finite α m]
-    [IteratorLoop α m m] [LawfulIteratorLoop α m m]
+theorem IterM.drain_eq_match_step {α β : Type w} {m : Type w → Type w'} [Iterator α m β] [Finite α m]
+    [Monad m] [LawfulMonad m] [IteratorLoop α m m] [LawfulIteratorLoop α m m]
     {it : IterM (α := α) m β} :
     it.drain = (do
-      match ← it.step with
-      | .yield it' _ => it'.drain
-      | .skip it' => it'.drain
-      | .done => return .unit) := by
+      match (← it.step).inflate with
+      | .yield it' _ _ => it'.drain
+      | .skip it' _ => it'.drain
+      | .done _ => return .unit) := by
   rw [IterM.drain_eq_fold, IterM.fold_eq_match_step]
   simp [IterM.drain_eq_fold]
 
-theorem IterM.drain_eq_map_toList {α β : Type w} {m : Type w → Type w'}
-    [Monad m] [MonadAttach m] [LawfulMonad m] [LawfulMonadAttach m]
-    [Iterator α m β] [Finite α m] [IteratorLoop α m m] [LawfulIteratorLoop α m m]
+theorem IterM.drain_eq_map_toList {α β : Type w} {m : Type w → Type w'} [Iterator α m β]
+    [Finite α m] [Monad m] [LawfulMonad m] [IteratorLoop α m m] [LawfulIteratorLoop α m m]
     [IteratorCollect α m m] [LawfulIteratorCollect α m m]
     {it : IterM (α := α) m β} :
     it.drain = (fun _ => .unit) <$> it.toList := by
   induction it using IterM.inductSteps with | step it ihy ihs
   rw [IterM.drain_eq_match_step, IterM.toList_eq_match_step]
   simp only [map_eq_pure_bind, bind_assoc]
-  simp only [← LawfulMonadAttach.map_attach (x := it.step), bind_map_left]
-  apply bind_congr; intro step
-  cases step using PlausibleIterStep.casesOn
+  apply bind_congr
+  intro step
+  cases step.inflate using PlausibleIterStep.casesOn
   · rename_i it' out h
     simp [ihy h]
   · rename_i it' h
     simp [ihs h]
   · simp
 
-theorem IterM.drain_eq_map_toListRev {α β : Type w} {m : Type w → Type w'}
-    [Monad m] [MonadAttach m] [LawfulMonad m] [LawfulMonadAttach m]
-    [Iterator α m β] [Finite α m] [IteratorLoop α m m] [LawfulIteratorLoop α m m]
+theorem IterM.drain_eq_map_toListRev {α β : Type w} {m : Type w → Type w'} [Iterator α m β]
+    [Finite α m] [Monad m] [LawfulMonad m] [IteratorLoop α m m] [LawfulIteratorLoop α m m]
     [IteratorCollect α m m] [LawfulIteratorCollect α m m]
     {it : IterM (α := α) m β} :
     it.drain = (fun _ => .unit) <$> it.toListRev := by
   simp [IterM.drain_eq_map_toList, IterM.toListRev_eq]
 
-theorem IterM.drain_eq_map_toArray {α β : Type w} {m : Type w → Type w'}
-    [Monad m] [MonadAttach m] [LawfulMonad m] [LawfulMonadAttach m]
-    [Iterator α m β] [Finite α m] [IteratorLoop α m m] [LawfulIteratorLoop α m m]
+theorem IterM.drain_eq_map_toArray {α β : Type w} {m : Type w → Type w'} [Iterator α m β]
+    [Finite α m] [Monad m] [LawfulMonad m] [IteratorLoop α m m] [LawfulIteratorLoop α m m]
     [IteratorCollect α m m] [LawfulIteratorCollect α m m]
     {it : IterM (α := α) m β} :
     it.drain = (fun _ => .unit) <$> it.toList := by
   simp [IterM.drain_eq_map_toList]
 
-theorem IterM.count_eq_fold {α β : Type w} {m : Type w → Type w'}
-    [Monad m] [MonadAttach m]
-    [Iterator α m β] [IteratorLoop α m m]
+theorem IterM.count_eq_fold {α β : Type w} {m : Type w → Type w'} [Iterator α m β]
+    [Finite α m] [Monad m] [LawfulMonad m] [IteratorLoop α m m]
     {it : IterM (α := α) m β} :
     it.count = it.fold (init := .up 0) (fun acc _ => .up <| acc.down + 1) :=
   (rfl)
 
-theorem IterM.count_eq_forIn {α β : Type w} {m : Type w → Type w'}
-    [Monad m] [MonadAttach m]
-    [Iterator α m β] [IteratorLoop α m m]
+theorem IterM.count_eq_forIn {α β : Type w} {m : Type w → Type w'} [Iterator α m β]
+    [Finite α m] [Monad m] [LawfulMonad m] [IteratorLoop α m m]
     {it : IterM (α := α) m β} :
     it.count = ForIn.forIn it (.up 0) (fun _ acc => return .yield (.up (acc.down + 1))) :=
   (rfl)
 
-theorem IterM.count_eq_match_step {α β : Type w} {m : Type w → Type w'}
-    [Monad m] [MonadAttach m] [LawfulMonad m] [LawfulMonadAttach m]
-    [Iterator α m β] [Finite α m] [IteratorLoop α m m] [LawfulIteratorLoop α m m]
+theorem IterM.count_eq_match_step {α β : Type w} {m : Type w → Type w'} [Iterator α m β]
+    [Finite α m] [Monad m] [LawfulMonad m] [IteratorLoop α m m] [LawfulIteratorLoop α m m]
     {it : IterM (α := α) m β} :
     it.count = (do
-      match ← it.step with
+      match (← it.step).inflate.val with
       | .yield it' _ => return .up ((← it'.count).down + 1)
       | .skip it' => return .up (← it'.count).down
       | .done => return .up 0) := by
@@ -497,18 +441,16 @@ theorem IterM.count_eq_match_step {α β : Type w} {m : Type w → Type w'}
     · simp only [Nat.zero_add]; rfl
     · simp only [ULift.up.injEq]; omega
   rw [fold_eq_match_step]
-  simp only [← LawfulMonadAttach.map_attach (x := it.step), bind_map_left]
   apply bind_congr; intro step
-  cases step using PlausibleIterStep.casesOn
+  cases step.inflate using PlausibleIterStep.casesOn
   · simp only [Nat.zero_add, bind_pure_comp]
     rw [this 1]
   · simp
   · simp
 
 @[simp]
-theorem IterM.up_size_toArray_eq_count {α β : Type w}
-    [Monad m] [MonadAttach m] [LawfulMonad m] [LawfulMonadAttach m]
-    [Iterator α m β] [Finite α m]
+theorem IterM.up_size_toArray_eq_count {α β : Type w} [Iterator α m β] [Finite α m]
+    [Monad m] [LawfulMonad m]
     [IteratorCollect α m m] [LawfulIteratorCollect α m m]
     [IteratorLoop α m m] [LawfulIteratorLoop α m m]
     {it : IterM (α := α) m β} :
@@ -518,9 +460,8 @@ theorem IterM.up_size_toArray_eq_count {α β : Type w}
   · simp
 
 @[simp]
-theorem IterM.up_length_toList_eq_count {α β : Type w}
-    [Monad m] [MonadAttach m] [LawfulMonad m] [LawfulMonadAttach m]
-    [Iterator α m β] [Finite α m]
+theorem IterM.up_length_toList_eq_count {α β : Type w} [Iterator α m β] [Finite α m]
+    [Monad m] [LawfulMonad m]
     [IteratorCollect α m m] [LawfulIteratorCollect α m m]
     [IteratorLoop α m m] [LawfulIteratorLoop α m m]
     {it : IterM (α := α) m β} :
@@ -530,18 +471,16 @@ theorem IterM.up_length_toList_eq_count {α β : Type w}
   · simp
 
 @[simp]
-theorem IterM.up_length_toListRev_eq_count {α β : Type w}
-    [Monad m] [MonadAttach m] [LawfulMonad m] [LawfulMonadAttach m]
-    [Iterator α m β] [Finite α m]
+theorem IterM.up_length_toListRev_eq_count {α β : Type w} [Iterator α m β] [Finite α m]
+    [Monad m] [LawfulMonad m]
     [IteratorCollect α m m] [LawfulIteratorCollect α m m]
     [IteratorLoop α m m] [LawfulIteratorLoop α m m]
     {it : IterM (α := α) m β} :
     (.up <| ·.length) <$> it.toListRev = it.count := by
   simp only [toListRev_eq, Functor.map_map, List.length_reverse, up_length_toList_eq_count]
 
-theorem IterM.anyM_eq_forIn {α β : Type w} {m : Type w → Type w'}
-    [Monad m] [MonadAttach m]
-    [Iterator α m β] [IteratorLoop α m m]
+theorem IterM.anyM_eq_forIn {α β : Type w} {m : Type w → Type w'} [Iterator α m β]
+    [Finite α m] [Monad m] [LawfulMonad m] [IteratorLoop α m m] [LawfulIteratorLoop α m m]
     {it : IterM (α := α) m β} {p : β → m (ULift Bool)} :
     it.anyM p = (ForIn.forIn it (.up false) (fun x _ => do
         if (← p x).down then
@@ -550,12 +489,11 @@ theorem IterM.anyM_eq_forIn {α β : Type w} {m : Type w → Type w'}
           return .yield (.up false))) := by
   rfl
 
-theorem IterM.anyM_eq_match_step {α β : Type w} {m : Type w → Type w'}
-    [Monad m] [MonadAttach m] [LawfulMonad m] [LawfulMonadAttach m]
-    [Iterator α m β] [Finite α m] [IteratorLoop α m m] [LawfulIteratorLoop α m m]
+theorem IterM.anyM_eq_match_step {α β : Type w} {m : Type w → Type w'} [Iterator α m β]
+    [Finite α m] [Monad m] [LawfulMonad m] [IteratorLoop α m m] [LawfulIteratorLoop α m m]
     {it : IterM (α := α) m β} {p : β → m (ULift Bool)} :
     it.anyM p = (do
-      match ← it.step with
+      match (← it.step).inflate.val with
       | .yield it' x =>
         if (← p x).down then
           return .up true
@@ -565,9 +503,8 @@ theorem IterM.anyM_eq_match_step {α β : Type w} {m : Type w → Type w'}
       | .done => return .up false) := by
   rw [anyM_eq_forIn, forIn_eq_match_step]
   simp only [monadLift_self, bind_assoc]
-  simp only [← LawfulMonadAttach.map_attach (x := it.step), bind_map_left]
   apply bind_congr; intro step
-  cases step using PlausibleIterStep.casesOn
+  cases step.inflate using PlausibleIterStep.casesOn
   · apply bind_congr; intro px
     split
     · simp
@@ -575,24 +512,23 @@ theorem IterM.anyM_eq_match_step {α β : Type w} {m : Type w → Type w'}
   · simp [anyM_eq_forIn]
   · simp
 
-theorem IterM.any_eq_anyM {α β : Type w} {m : Type w → Type w'}
-    [Monad m] [MonadAttach m] [Iterator α m β] [IteratorLoop α m m]
+theorem IterM.any_eq_anyM {α β : Type w} {m : Type w → Type w'} [Iterator α m β]
+    [Finite α m] [Monad m] [LawfulMonad m] [IteratorLoop α m m] [LawfulIteratorLoop α m m]
     {it : IterM (α := α) m β} {p : β → Bool} :
     it.any p = it.anyM (fun x => pure (.up (p x))) := by
   rfl
 
-theorem IterM.anyM_pure {α β : Type w} {m : Type w → Type w'}
-    [Monad m] [MonadAttach m] [Iterator α m β] [IteratorLoop α m m]
+theorem IterM.anyM_pure {α β : Type w} {m : Type w → Type w'} [Iterator α m β]
+    [Finite α m] [Monad m] [LawfulMonad m] [IteratorLoop α m m] [LawfulIteratorLoop α m m]
     {it : IterM (α := α) m β} {p : β → ULift Bool} :
     it.anyM (fun x => pure (p x)) = it.any (fun x => (p x).down) := by
   simp [any_eq_anyM]
 
-theorem IterM.any_eq_match_step {α β : Type w} {m : Type w → Type w'}
-    [Monad m] [MonadAttach m] [LawfulMonad m] [LawfulMonadAttach m]
-    [Iterator α m β] [Finite α m] [IteratorLoop α m m] [LawfulIteratorLoop α m m]
+theorem IterM.any_eq_match_step {α β : Type w} {m : Type w → Type w'} [Iterator α m β]
+    [Finite α m] [Monad m] [LawfulMonad m] [IteratorLoop α m m] [LawfulIteratorLoop α m m]
     {it : IterM (α := α) m β} {p : β → Bool} :
     it.any p = (do
-      match ← it.step with
+      match (← it.step).inflate.val with
       | .yield it' x =>
         if p x then
           return .up true
@@ -607,9 +543,8 @@ theorem IterM.any_eq_match_step {α β : Type w} {m : Type w → Type w'}
   · simp [any_eq_anyM]
   · simp
 
-theorem IterM.any_eq_forIn {α β : Type w} {m : Type w → Type w'}
-    [Monad m] [MonadAttach m] [LawfulMonad m] [LawfulMonadAttach m]
-    [Iterator α m β] [Finite α m] [IteratorLoop α m m] [LawfulIteratorLoop α m m]
+theorem IterM.any_eq_forIn {α β : Type w} {m : Type w → Type w'} [Iterator α m β]
+    [Finite α m] [Monad m] [LawfulMonad m] [IteratorLoop α m m] [LawfulIteratorLoop α m m]
     {it : IterM (α := α) m β} {p : β → Bool} :
     it.any p = (ForIn.forIn it (.up false) (fun x _ => do
         if p x then
@@ -618,9 +553,8 @@ theorem IterM.any_eq_forIn {α β : Type w} {m : Type w → Type w'}
           return .yield (.up false))) := by
   simp [any_eq_anyM, anyM_eq_forIn]
 
-theorem IterM.allM_eq_forIn {α β : Type w} {m : Type w → Type w'}
-    [Monad m] [MonadAttach m]
-    [Iterator α m β] [Finite α m] [IteratorLoop α m m]
+theorem IterM.allM_eq_forIn {α β : Type w} {m : Type w → Type w'} [Iterator α m β]
+    [Finite α m] [Monad m] [LawfulMonad m] [IteratorLoop α m m] [LawfulIteratorLoop α m m]
     {it : IterM (α := α) m β} {p : β → m (ULift Bool)} :
     it.allM p = (ForIn.forIn it (.up true) (fun x _ => do
         if (← p x).down then
@@ -629,12 +563,11 @@ theorem IterM.allM_eq_forIn {α β : Type w} {m : Type w → Type w'}
           return .done (.up false))) := by
   rfl
 
-theorem IterM.allM_eq_match_step {α β : Type w} {m : Type w → Type w'}
-    [Monad m] [MonadAttach m] [LawfulMonad m] [LawfulMonadAttach m]
-    [Iterator α m β] [Finite α m] [IteratorLoop α m m] [LawfulIteratorLoop α m m]
+theorem IterM.allM_eq_match_step {α β : Type w} {m : Type w → Type w'} [Iterator α m β]
+    [Finite α m] [Monad m] [LawfulMonad m] [IteratorLoop α m m] [LawfulIteratorLoop α m m]
     {it : IterM (α := α) m β} {p : β → m (ULift Bool)} :
     it.allM p = (do
-      match ← it.step with
+      match (← it.step).inflate.val with
       | .yield it' x =>
         if (← p x).down then
           it'.allM p
@@ -644,9 +577,8 @@ theorem IterM.allM_eq_match_step {α β : Type w} {m : Type w → Type w'}
       | .done => return .up true) := by
   rw [allM_eq_forIn, forIn_eq_match_step]
   simp only [monadLift_self, bind_assoc]
-  simp only [← LawfulMonadAttach.map_attach (x := it.step), bind_map_left]
   apply bind_congr; intro step
-  cases step using PlausibleIterStep.casesOn
+  cases step.inflate using PlausibleIterStep.casesOn
   · apply bind_congr; intro px
     split
     · simp [allM_eq_forIn]
@@ -654,26 +586,23 @@ theorem IterM.allM_eq_match_step {α β : Type w} {m : Type w → Type w'}
   · simp [allM_eq_forIn]
   · simp
 
-theorem IterM.all_eq_allM {α β : Type w} {m : Type w → Type w'}
-    [Monad m] [MonadAttach m]
-    [Iterator α m β] [IteratorLoop α m m]
+theorem IterM.all_eq_allM {α β : Type w} {m : Type w → Type w'} [Iterator α m β]
+    [Finite α m] [Monad m] [LawfulMonad m] [IteratorLoop α m m] [LawfulIteratorLoop α m m]
     {it : IterM (α := α) m β} {p : β → Bool} :
     it.all p = it.allM (fun x => pure (.up (p x))) := by
   rfl
 
-theorem IterM.allM_pure {α β : Type w} {m : Type w → Type w'}
-    [Monad m] [MonadAttach m]
-    [Iterator α m β] [IteratorLoop α m m]
+theorem IterM.allM_pure {α β : Type w} {m : Type w → Type w'} [Iterator α m β]
+    [Finite α m] [Monad m] [LawfulMonad m] [IteratorLoop α m m] [LawfulIteratorLoop α m m]
     {it : IterM (α := α) m β} {p : β → ULift Bool} :
     it.allM (fun x => pure (p x)) = it.all (fun x => (p x).down) := by
   simp [all_eq_allM]
 
-theorem IterM.all_eq_match_step {α β : Type w} {m : Type w → Type w'}
-    [Monad m] [MonadAttach m] [LawfulMonad m] [LawfulMonadAttach m]
-    [Iterator α m β] [Finite α m] [IteratorLoop α m m] [LawfulIteratorLoop α m m]
+theorem IterM.all_eq_match_step {α β : Type w} {m : Type w → Type w'} [Iterator α m β]
+    [Finite α m] [Monad m] [LawfulMonad m] [IteratorLoop α m m] [LawfulIteratorLoop α m m]
     {it : IterM (α := α) m β} {p : β → Bool} :
     it.all p = (do
-      match ← it.step with
+      match (← it.step).inflate.val with
       | .yield it' x =>
         if p x then
           it'.all p
@@ -688,9 +617,8 @@ theorem IterM.all_eq_match_step {α β : Type w} {m : Type w → Type w'}
   · simp [all_eq_allM]
   · simp
 
-theorem IterM.all_eq_forIn {α β : Type w} {m : Type w → Type w'}
-    [Monad m] [MonadAttach m] [LawfulMonad m] [LawfulMonadAttach m]
-    [Iterator α m β] [Finite α m] [IteratorLoop α m m] [LawfulIteratorLoop α m m]
+theorem IterM.all_eq_forIn {α β : Type w} {m : Type w → Type w'} [Iterator α m β]
+    [Finite α m] [Monad m] [LawfulMonad m] [IteratorLoop α m m] [LawfulIteratorLoop α m m]
     {it : IterM (α := α) m β} {p : β → Bool} :
     it.all p = (ForIn.forIn it (.up true) (fun x _ => do
         if p x then
@@ -699,17 +627,15 @@ theorem IterM.all_eq_forIn {α β : Type w} {m : Type w → Type w'}
           return .done (.up false))) := by
   simp [all_eq_allM, allM_eq_forIn]
 
-theorem IterM.allM_eq_not_anyM_not {α β : Type w} {m : Type w → Type w'}
-    [Monad m] [MonadAttach m] [LawfulMonad m] [LawfulMonadAttach m]
-    [Iterator α m β] [Finite α m] [IteratorLoop α m m] [LawfulIteratorLoop α m m]
+theorem IterM.allM_eq_not_anyM_not {α β : Type w} {m : Type w → Type w'} [Iterator α m β]
+    [Finite α m] [Monad m] [LawfulMonad m] [IteratorLoop α m m] [LawfulIteratorLoop α m m]
     {it : IterM (α := α) m β} {p : β → m (ULift Bool)} :
     it.allM p = (fun x => .up !x.down) <$> it.anyM ((fun x => .up !x.down) <$> p ·) := by
   induction it using IterM.inductSteps with | step it ihy ihs =>
   rw [allM_eq_match_step, anyM_eq_match_step, map_eq_pure_bind, bind_assoc]
-  simp only [← LawfulMonadAttach.map_attach (x := it.step), bind_map_left]
   apply bind_congr; intro step
-  cases step using PlausibleIterStep.casesOn
-  · simp only [map_eq_pure_bind, bind_assoc]
+  cases step.inflate using PlausibleIterStep.casesOn
+  · simp only [map_eq_pure_bind, bind_assoc, pure_bind]
     apply bind_congr; intro px
     split
     · simp [*, ihy ‹_›]
@@ -717,16 +643,14 @@ theorem IterM.allM_eq_not_anyM_not {α β : Type w} {m : Type w → Type w'}
   · simp [ihs ‹_›]
   · simp
 
-theorem IterM.all_eq_not_any_not {α β : Type w} {m : Type w → Type w'}
-    [Monad m] [MonadAttach m] [LawfulMonad m] [LawfulMonadAttach m]
-    [Iterator α m β] [Finite α m] [IteratorLoop α m m] [LawfulIteratorLoop α m m]
+theorem IterM.all_eq_not_any_not {α β : Type w} {m : Type w → Type w'} [Iterator α m β]
+    [Finite α m] [Monad m] [LawfulMonad m] [IteratorLoop α m m] [LawfulIteratorLoop α m m]
     {it : IterM (α := α) m β} {p : β → Bool} :
     it.all p = (fun x => .up !x.down) <$> it.any (! p ·) := by
   induction it using IterM.inductSteps with | step it ihy ihs =>
   rw [all_eq_match_step, any_eq_match_step, map_eq_pure_bind, bind_assoc]
-  simp only [← LawfulMonadAttach.map_attach (x := it.step), bind_map_left]
   apply bind_congr; intro step
-  cases step using PlausibleIterStep.casesOn
+  cases step.inflate using PlausibleIterStep.casesOn
   · simp only
     split
     · simp [*, ihy ‹_›]
@@ -734,12 +658,11 @@ theorem IterM.all_eq_not_any_not {α β : Type w} {m : Type w → Type w'}
   · simp [ihs ‹_›]
   · simp
 
-theorem IterM.findSomeM?_eq_match_step {α β γ : Type w} {m : Type w → Type w'}
-    [Monad m] [MonadAttach m] [LawfulMonad m] [LawfulMonadAttach m]
-    [Iterator α m β] [IteratorLoop α m m] [Finite α m] [LawfulIteratorLoop α m m]
+theorem IterM.findSomeM?_eq_match_step {α β γ : Type w} {m : Type w → Type w'} [Monad m]
+    [Iterator α m β] [IteratorLoop α m m] [LawfulMonad m] [Finite α m] [LawfulIteratorLoop α m m]
     {it : IterM (α := α) m β} {f : β → m (Option γ)} :
     it.findSomeM? f = (do
-      match ← it.step with
+      match (← it.step).inflate.val with
       | .yield it' out =>
         match ← f out with
         | none => it'.findSomeM? f
@@ -747,28 +670,25 @@ theorem IterM.findSomeM?_eq_match_step {α β γ : Type w} {m : Type w → Type 
       | .skip it' => it'.findSomeM? f
       | .done => return none) := by
   rw [findSomeM?, forIn_eq_match_step]
-  simp only [← LawfulMonadAttach.map_attach (x := it.step), liftM_map, bind_map_left]
   apply bind_congr; intro step
-  cases step using PlausibleIterStep.casesOn
+  cases step.inflate using PlausibleIterStep.casesOn
   · simp only [bind_assoc]
     apply bind_congr; intro fx
     split <;> simp [findSomeM?]
   · simp [findSomeM?]
   · simp
 
-theorem IterM.findSome?_eq_findSomeM? {α β γ : Type w} {m : Type w → Type w'}
-    [Monad m] [MonadAttach m]
-    [Iterator α m β] [IteratorLoop α m m]
+theorem IterM.findSome?_eq_findSomeM? {α β γ : Type w} {m : Type w → Type w'} [Monad m]
+    [Iterator α m β] [IteratorLoop α m m] [Finite α m]
     {it : IterM (α := α) m β} {f : β → Option γ} :
     it.findSome? f = it.findSomeM? (pure <| f ·) :=
   (rfl)
 
-theorem IterM.findSome?_eq_match_step {α β γ : Type w} {m : Type w → Type w'}
-    [Monad m] [MonadAttach m] [LawfulMonad m] [LawfulMonadAttach m]
-    [Iterator α m β] [IteratorLoop α m m] [Finite α m] [LawfulIteratorLoop α m m]
+theorem IterM.findSome?_eq_match_step {α β γ : Type w} {m : Type w → Type w'} [Monad m]
+    [Iterator α m β] [IteratorLoop α m m] [LawfulMonad m] [Finite α m] [LawfulIteratorLoop α m m]
     {it : IterM (α := α) m β} {f : β → Option γ} :
     it.findSome? f = (do
-      match ← it.step with
+      match (← it.step).inflate.val with
       | .yield it' out =>
         match f out with
         | none => it'.findSome? f
@@ -779,35 +699,31 @@ theorem IterM.findSome?_eq_match_step {α β γ : Type w} {m : Type w → Type w
   apply bind_congr; intro step
   split <;> simp [findSome?_eq_findSomeM?]
 
-theorem IterM.findSomeM?_pure {α β γ : Type w} {m : Type w → Type w'}
-    [Monad m] [MonadAttach m] [LawfulMonad m] [LawfulMonadAttach m]
+theorem IterM.findSomeM?_pure {α β γ : Type w} {m : Type w → Type w'} [Monad m]
     [Iterator α m β] [IteratorLoop α m m]
-    [Finite α m] [LawfulIteratorLoop α m m]
+    [LawfulMonad m] [Finite α m] [LawfulIteratorLoop α m m]
     {it : IterM (α := α) m β} {f : β → Option γ} :
     it.findSomeM? (pure <| f ·) = it.findSome? f := by
   induction it using IterM.inductSteps with | step it ihy ihs
   rw [findSomeM?_eq_match_step, findSome?_eq_match_step]
-  simp only [← LawfulMonadAttach.map_attach (x := it.step), bind_map_left]
   apply bind_congr; intro step
-  cases step using PlausibleIterStep.casesOn
+  cases step.inflate using PlausibleIterStep.casesOn
   · simp only [pure_bind]
     split <;> simp [ihy ‹_›]
   · simp [ihs ‹_›]
   · simp
 
-theorem IterM.findM?_eq_findSomeM? {α β : Type w} {m : Type w → Type w'}
-    [Monad m] [MonadAttach m]
-    [Iterator α m β] [IteratorLoop α m m]
+theorem IterM.findM?_eq_findSomeM? {α β : Type w} {m : Type w → Type w'} [Monad m]
+    [Iterator α m β] [IteratorLoop α m m] [Finite α m]
     {it : IterM (α := α) m β} {f : β → m (ULift Bool)} :
     it.findM? f = it.findSomeM? (fun x => return if (← f x).down then some x else none) :=
   (rfl)
 
-theorem IterM.findM?_eq_match_step {α β : Type w} {m : Type w → Type w'}
-    [Monad m] [MonadAttach m] [LawfulMonad m] [LawfulMonadAttach m]
-    [Iterator α m β] [IteratorLoop α m m] [Finite α m] [LawfulIteratorLoop α m m]
+theorem IterM.findM?_eq_match_step {α β : Type w} {m : Type w → Type w'} [Monad m]
+    [Iterator α m β] [IteratorLoop α m m] [LawfulMonad m] [Finite α m] [LawfulIteratorLoop α m m]
     {it : IterM (α := α) m β} {f : β → m (ULift Bool)} :
     it.findM? f = (do
-      match ← it.step with
+      match (← it.step).inflate.val with
       | .yield it' out =>
         if (← f out).down then return (some out) else it'.findM? f
       | .skip it' => it'.findM? f
@@ -821,24 +737,21 @@ theorem IterM.findM?_eq_match_step {α β : Type w} {m : Type w → Type w'}
   · simp [findM?_eq_findSomeM?]
   · simp
 
-theorem IterM.find?_eq_findM? {α β : Type w} {m : Type w → Type w'}
-    [Monad m] [MonadAttach m]
-    [Iterator α m β] [IteratorLoop α m m] {it : IterM (α := α) m β} {f : β → Bool} :
+theorem IterM.find?_eq_findM? {α β : Type w} {m : Type w → Type w'} [Monad m] [Iterator α m β]
+    [IteratorLoop α m m] [Finite α m] {it : IterM (α := α) m β} {f : β → Bool} :
     it.find? f = it.findM? (pure <| .up <| f ·) :=
   (rfl)
 
-theorem IterM.find?_eq_findSome? {α β : Type w} {m : Type w → Type w'}
-    [Monad m] [MonadAttach m] [LawfulMonad m] [LawfulMonadAttach m]
-    [Iterator α m β] [IteratorLoop α m m] [Finite α m] {it : IterM (α := α) m β} {f : β → Bool} :
+theorem IterM.find?_eq_findSome? {α β : Type w} {m : Type w → Type w'} [Monad m] [Iterator α m β]
+    [IteratorLoop α m m] [LawfulMonad m] [Finite α m] {it : IterM (α := α) m β} {f : β → Bool} :
     it.find? f = it.findSome? (fun x => if f x then some x else none) := by
   simp [find?_eq_findM?, findSome?_eq_findSomeM?, findM?_eq_findSomeM?]
 
-theorem IterM.find?_eq_match_step {α β : Type w} {m : Type w → Type w'}
-    [Monad m] [MonadAttach m] [LawfulMonad m] [LawfulMonadAttach m]
-    [Iterator α m β] [IteratorLoop α m m] [Finite α m] [LawfulIteratorLoop α m m]
+theorem IterM.find?_eq_match_step {α β : Type w} {m : Type w → Type w'} [Monad m]
+    [Iterator α m β] [IteratorLoop α m m] [LawfulMonad m] [Finite α m] [LawfulIteratorLoop α m m]
     {it : IterM (α := α) m β} {f : β → Bool} :
     it.find? f = (do
-      match ← it.step with
+      match (← it.step).inflate.val with
       | .yield it' out =>
         if f out then return (some out) else it'.find? f
       | .skip it' => it'.find? f
@@ -851,17 +764,15 @@ theorem IterM.find?_eq_match_step {α β : Type w} {m : Type w → Type w'}
   · simp [find?_eq_findM?]
   · simp
 
-theorem IterM.findM?_pure {α β : Type w} {m : Type w → Type w'}
-    [Monad m] [MonadAttach m] [LawfulMonad m] [LawfulMonadAttach m]
+theorem IterM.findM?_pure {α β : Type w} {m : Type w → Type w'} [Monad m]
     [Iterator α m β] [IteratorLoop α m m]
-    [Finite α m] [LawfulIteratorLoop α m m]
+    [LawfulMonad m] [Finite α m] [LawfulIteratorLoop α m m]
     {it : IterM (α := α) m β} {f : β → ULift Bool} :
     it.findM? (pure (f := m) <| f ·) = it.find? (ULift.down <| f ·) := by
   induction it using IterM.inductSteps with | step it ihy ihs
   rw [findM?_eq_match_step, find?_eq_match_step]
-  simp only [← LawfulMonadAttach.map_attach (x := it.step), bind_map_left]
   apply bind_congr; intro step
-  cases step using PlausibleIterStep.casesOn
+  cases step.inflate using PlausibleIterStep.casesOn
   · simp only [pure_bind]
     split
     · simp
