src/Std/Data/Iterators/Combinators/Monadic/StepSize.lean
@@ -8,10 +8,8 @@ module
 prelude
 public import Init.Data.Iterators.Internal.Termination
 public import Init.Data.Iterators.Consumers.Monadic.Access
-import all Init.Data.Iterators.Consumers.Monadic.Access
 public import Init.Data.Iterators.Consumers.Monadic.Collect
 public import Init.Data.Iterators.Consumers.Monadic.Loop
-import Init.Control.Lawful.MonadAttach.Lemmas
 
 @[expose] public section
 
@@ -27,15 +25,28 @@ structure Types.StepSizeIterator (α : Type w) (m : Type w → Type w') (β : Ty
   n : Nat
   inner : IterM (α := α) m β
 
-instance
-    [Monad m] [Iterator α m β] [IteratorAccess α m] :
+instance [Iterator α m β] [IteratorAccess α m] [Monad m] :
     Iterator (Types.StepSizeIterator α m β) m β where
-  step it := (fun s => s.mapIterator (⟨⟨it.internalState.n, it.internalState.n, ·⟩⟩)) <$>
-    it.internalState.inner.nextAtIdx? it.internalState.nextIdx
+  IsPlausibleStep it step :=
+    it.internalState.inner.IsPlausibleNthOutputStep it.internalState.nextIdx
+        (step.mapIterator (Types.StepSizeIterator.inner ∘ IterM.internalState)) ∧
+      ∀ it' out, step = .yield it' out →
+        it'.internalState.n = it.internalState.n ∧ it'.internalState.nextIdx = it.internalState.n
+  step it := (fun s => .deflate ⟨s.1.mapIterator (⟨⟨it.internalState.n, it.internalState.n, ·⟩⟩), by
+      simp only [IterStep.mapIterator_mapIterator]
+      refine cast ?_ s.property
+      rw (occs := [1]) [← IterStep.mapIterator_id (step := s.val)]
+      congr, by
+      intro it' out
+      cases s.val
+      · simp only [IterStep.mapIterator_yield, IterStep.yield.injEq, and_imp]
+        rintro h _
+        simp [← h]
+      · simp
+      · simp
+      done⟩) <$> it.internalState.inner.nextAtIdx? it.internalState.nextIdx
 
-def Types.StepSizeIterator.instFinitenessRelation
-    [Monad m] [MonadAttach m] [LawfulMonad m] [LawfulMonadAttach m]
-    [Iterator α m β] [IteratorAccess α m] [LawfulIteratorAccess α m]
+def Types.StepSizeIterator.instFinitenessRelation [Iterator α m β] [IteratorAccess α m] [Monad m]
     [Finite α m] : FinitenessRelation (Types.StepSizeIterator α m β) m where
   rel := InvImage WellFoundedRelation.rel (fun it => it.internalState.inner.finitelyManySteps)
   wf := by
@@ -43,53 +54,54 @@ def Types.StepSizeIterator.instFinitenessRelation
     apply WellFoundedRelation.wf
   subrelation {it it'} h := by
     obtain ⟨step, hs, h⟩ := h
-    obtain ⟨step', hs', rfl⟩ := LawfulMonadAttach.canReturn_map_imp' h
-    replace hs' := LawfulIteratorAccess.isPlausibleNthOutputStep_of_canReturn hs'
-    clear h
+    simp only [IterM.IsPlausibleStep, Iterator.IsPlausibleStep] at h
+    simp only [InvImage]
     obtain ⟨⟨n, it⟩⟩ := it
-    simp only at ⊢ hs'
-    induction hs'
+    simp only at ⊢ h
+    generalize h' : step.mapIterator (Types.StepSizeIterator.inner ∘ IterM.internalState) = s at h
+    replace h := h.1
+    induction h
     case zero_yield =>
-      cases hs
-      exact IterM.TerminationMeasures.Finite.rel_of_yield ‹_›
+      cases step <;> (try exfalso; simp at h'; done)
+      cases hs; cases h'
+      apply IterM.TerminationMeasures.Finite.rel_of_yield ‹_›
     case done =>
-      simp_all [IterStep.successor]
+      cases step <;> simp_all [IterStep.successor]
     case yield ih =>
       apply Relation.TransGen.trans
-      · exact ih hs
+      · exact ih h'
       · exact IterM.TerminationMeasures.Finite.rel_of_yield ‹_›
     case skip ih  =>
       apply Relation.TransGen.trans
-      · exact ih hs
+      · exact ih h'
       · exact IterM.TerminationMeasures.Finite.rel_of_skip ‹_›
 
-instance Types.StepSizeIterator.instFinite
-    [Monad m] [MonadAttach m] [LawfulMonad m] [LawfulMonadAttach m]
-    [Iterator α m β] [IteratorAccess α m] [LawfulIteratorAccess α m] [Finite α m] :
-    Finite (Types.StepSizeIterator α m β) m :=
+instance Types.StepSizeIterator.instFinite [Iterator α m β] [IteratorAccess α m] [Monad m]
+    [Finite α m] : Finite (Types.StepSizeIterator α m β) m :=
   .of_finitenessRelation instFinitenessRelation
 
-def Types.StepSizeIterator.instProductivenessRelation
-    [Monad m] [MonadAttach m] [LawfulMonad m] [LawfulMonadAttach m]
-    [Iterator α m β] [IteratorAccess α m] [LawfulIteratorAccess α m] [Productive α m] :
-    ProductivenessRelation (Types.StepSizeIterator α m β) m where
+def Types.StepSizeIterator.instProductivenessRelation [Iterator α m β] [IteratorAccess α m] [Monad m]
+    [Productive α m] : ProductivenessRelation (Types.StepSizeIterator α m β) m where
   rel := InvImage WellFoundedRelation.rel (fun it => it.internalState.inner.finitelyManySkips)
   wf := by
     apply InvImage.wf
     apply WellFoundedRelation.wf
   subrelation {it it'} h := by
-    obtain ⟨step', hs', h'⟩ := LawfulMonadAttach.canReturn_map_imp' h
-    replace hs' := LawfulIteratorAccess.isPlausibleNthOutputStep_of_canReturn hs'
-    cases step'
-    · cases h'
-    · exfalso
-      exact IterM.not_isPlausibleNthOutputStep_skip hs'
-    · cases h'
+    simp only [IterM.IsPlausibleSkipSuccessorOf, IterM.IsPlausibleStep, Iterator.IsPlausibleStep] at h
+    simp only [InvImage]
+    obtain ⟨⟨n, it⟩⟩ := it
+    simp only [IterStep.mapIterator_skip, Function.comp_apply] at ⊢ h
+    generalize h' : IterStep.skip _ = s at h
+    exfalso
+    replace h := h.1
+    induction h
+    case zero_yield => cases h'
+    case done => cases h'
+    case yield hp ih => exact ih h'
+    case skip ih  => exact ih h'
 
-instance Types.StepSizeIterator.instProductive
-    [Monad m] [MonadAttach m] [LawfulMonad m] [LawfulMonadAttach m]
-    [Iterator α m β] [IteratorAccess α m] [LawfulIteratorAccess α m] [Productive α m] :
-    Productive (Types.StepSizeIterator α m β) m :=
+instance Types.StepSizeIterator.instProductive [Iterator α m β] [IteratorAccess α m] [Monad m]
+    [Productive α m] : Productive (Types.StepSizeIterator α m β) m :=
   .of_productivenessRelation instProductivenessRelation
 
 /--
@@ -123,12 +135,12 @@ def IterM.stepSize [Iterator α m β] [IteratorAccess α m] [Monad m]
   ⟨⟨0, n - 1, it⟩⟩
 
 instance Types.StepSizeIterator.instIteratorCollect {m n} [Iterator α m β]
-    [IteratorAccess α m] [Monad m] [MonadAttach m] [Monad n] :
+    [IteratorAccess α m] [Monad m] [Monad n] :
     IteratorCollect (Types.StepSizeIterator α m β) m n :=
   .defaultImplementation
 
 instance Types.StepSizeIterator.instIteratorLoop {m n} [Iterator α m β]
-    [IteratorAccess α m] [Monad m] [MonadAttach m] [MonadAttach n] [Monad n] :
+    [IteratorAccess α m] [Monad m] [Monad n] :
     IteratorLoop (Types.StepSizeIterator α m β) m n :=
   .defaultImplementation
 
