src/Std/Data/Iterators/Combinators/Monadic/TakeWhile.lean
@@ -11,7 +11,6 @@ public import Init.Data.Iterators.Consumers.Monadic.Collect
 public import Init.Data.Iterators.Consumers.Monadic.Loop
 public import Init.Data.Iterators.Internal.Termination
 public import Init.Data.Iterators.PostconditionMonad
-public import Init.Control.Lawful.MonadAttach.Lemmas
 
 @[expose] public section
 
@@ -27,6 +26,9 @@ Several variants of this combinator are provided:
 * `M` suffix: Instead of a pure function, this variant takes a monadic function. Given a suitable
   `MonadLiftT` instance, it will also allow lifting the iterator to another monad first and then
   applying the mapping function in this monad.
+* `WithPostcondition` suffix: This variant takes a monadic function where the return type in the
+  monad is a subtype. This variant is in rare cases necessary for the intrinsic verification of an
+  iterator, and particularly for specialized termination proofs. If possible, avoid this.
 -/
 
 namespace Std.Iterators
@@ -38,9 +40,52 @@ Internal state of the `takeWhile` combinator. Do not depend on its internals.
 -/
 @[unbox]
 structure TakeWhile (α : Type w) (m : Type w → Type w') (β : Type w)
-    (P : β → m (ULift Bool)) where
+    (P : β → PostconditionT m (ULift Bool)) where
   /-- Internal implementation detail of the iterator library. -/
   inner : IterM (α := α) m β
+
+/--
+*Note: This is a very general combinator that requires an advanced understanding of monads,
+dependent types and termination proofs. The variants `takeWhile` and `takeWhileM` are easier to use
+and sufficient for most use cases.*
+
+Given an iterator `it` and a monadic predicate `P`, `it.takeWhileWithPostcondition P` is an iterator
+that emits the values emitted by `it` until one of those values is rejected by `P`.
+If some emitted value is rejected by `P`, the value is dropped and the iterator terminates.
+
+`P` is expected to return `PostconditionT m (ULift Bool)`. The `PostconditionT` transformer allows
+the caller to intrinsically prove properties about `P`'s return value in the monad `m`, enabling
+termination proofs depending on the specific behavior of `P`.
+
+**Marble diagram (ignoring monadic effects):**
+
+Assuming that the predicate `P` accepts `a` and `b` but rejects `c`:
+
+```text
+it                                ---a----b---c--d-e--⊥
+it.takeWhileWithPostcondition P   ---a----b---⊥
+
+it                                ---a----⊥
+it.takeWhileWithPostcondition P   ---a----⊥
+```
+
+**Termination properties:**
+
+* `Finite` instance: only if `it` is finite
+* `Productive` instance: only if `it` is productive
+
+Depending on `P`, it is possible that `it.takeWhileWithPostcondition P` is finite (or productive)
+although `it` is not. In this case, the `Finite` (or `Productive`) instance needs to be proved
+manually.
+
+**Performance:**
+
+This combinator calls `P` on each output of `it` until the predicate evaluates to false. Then
+it terminates.
+-/
+@[always_inline, inline]
+def IterM.takeWhileWithPostcondition (P : β → PostconditionT m (ULift Bool)) (it : IterM (α := α) m β) :=
+  (toIterM (TakeWhile.mk (P := P) it) m β : IterM m β)
 
 /--
 Given an iterator `it` and a monadic predicate `P`, `it.takeWhileM P` is an iterator that outputs
@@ -75,9 +120,8 @@ This combinator calls `P` on each output of `it` until the predicate evaluates t
 it terminates.
 -/
 @[always_inline, inline]
-def IterM.takeWhileM [Monad m] (P : β → m (ULift Bool)) (it : IterM (α := α) m β) :
-    IterM (α := TakeWhile α m β P) m β :=
-  toIterM ⟨it⟩ m β
+def IterM.takeWhileM [Monad m] (P : β → m (ULift Bool)) (it : IterM (α := α) m β) :=
+  (it.takeWhileWithPostcondition (PostconditionT.lift ∘ P) : IterM m β)
 
 /--
 Given an iterator `it` and a predicate `P`, `it.takeWhile P` is an iterator that outputs
@@ -115,95 +159,79 @@ it terminates.
 def IterM.takeWhile [Monad m] (P : β → Bool) (it : IterM (α := α) m β) :=
   (it.takeWhileM (pure ∘ ULift.up ∘ P) : IterM m β)
 
--- /--
--- `it.PlausibleStep step` is the proposition that `step` is a possible next step from the
--- `takeWhile` iterator `it`. This is mostly internally relevant, except if one needs to manually
--- prove termination (`Finite` or `Productive` instances, for example) of a `takeWhile` iterator.
--- -/
--- inductive TakeWhile.PlausibleStep [MonadAttach m] [Iterator α m β] {P}
---     (it : IterM (α := TakeWhile α m β P) m β) :
---     (step : IterStep (IterM (α := TakeWhile α m β P) m β) β) → Prop where
---   | yield : ∀ {it' out}, it.internalState.inner.IsPlausibleStep (.yield it' out) →
---       (P out).Property (.up true) → PlausibleStep it (.yield (it'.takeWhileWithPostcondition P) out)
---   | skip : ∀ {it'}, it.internalState.inner.IsPlausibleStep (.skip it') →
---       PlausibleStep it (.skip (it'.takeWhileWithPostcondition P))
---   | done : it.internalState.inner.IsPlausibleStep .done → PlausibleStep it .done
---   | rejected : ∀ {it' out}, it.internalState.inner.IsPlausibleStep (.yield it' out) →
---       (P out).Property (.up false) → PlausibleStep it .done
+/--
+`it.PlausibleStep step` is the proposition that `step` is a possible next step from the
+`takeWhile` iterator `it`. This is mostly internally relevant, except if one needs to manually
+prove termination (`Finite` or `Productive` instances, for example) of a `takeWhile` iterator.
+-/
+inductive TakeWhile.PlausibleStep [Iterator α m β] {P} (it : IterM (α := TakeWhile α m β P) m β) :
+    (step : IterStep (IterM (α := TakeWhile α m β P) m β) β) → Prop where
+  | yield : ∀ {it' out}, it.internalState.inner.IsPlausibleStep (.yield it' out) →
+      (P out).Property (.up true) → PlausibleStep it (.yield (it'.takeWhileWithPostcondition P) out)
+  | skip : ∀ {it'}, it.internalState.inner.IsPlausibleStep (.skip it') →
+      PlausibleStep it (.skip (it'.takeWhileWithPostcondition P))
+  | done : it.internalState.inner.IsPlausibleStep .done → PlausibleStep it .done
+  | rejected : ∀ {it' out}, it.internalState.inner.IsPlausibleStep (.yield it' out) →
+      (P out).Property (.up false) → PlausibleStep it .done
 
 @[always_inline, inline]
 instance TakeWhile.instIterator [Monad m] [Iterator α m β] {P} :
     Iterator (TakeWhile α m β P) m β where
+  IsPlausibleStep := TakeWhile.PlausibleStep
   step it := do
-    match ← it.internalState.inner.step with
-    | .yield it' out => return match ← P out with
-      | .up true => .yield (it'.takeWhileM P) out
-      | .up false => .done
-    | .skip it' => return .skip (it'.takeWhileM P)
-    | .done => return .done
+    match (← it.internalState.inner.step).inflate with
+    | .yield it' out h => match ← (P out).operation with
+      | ⟨.up true, h'⟩ => pure <| .deflate <| .yield (it'.takeWhileWithPostcondition P) out (.yield h h')
+      | ⟨.up false, h'⟩ => pure <| .deflate <| .done (.rejected h h')
+    | .skip it' h => pure <| .deflate <| .skip (it'.takeWhileWithPostcondition P) (.skip h)
+    | .done h => pure <| .deflate <| .done (.done h)
 
-private def TakeWhile.instFinitenessRelation
-    [Monad m] [MonadAttach m] [LawfulMonad m] [LawfulMonadAttach m]
-    [Iterator α m β] [Finite α m] {P} : FinitenessRelation (TakeWhile α m β P) m where
+private def TakeWhile.instFinitenessRelation [Monad m] [Iterator α m β]
+    [Finite α m] {P} :
+    FinitenessRelation (TakeWhile α m β P) m where
   rel := InvImage WellFoundedRelation.rel (IterM.finitelyManySteps ∘ TakeWhile.inner ∘ IterM.internalState)
   wf := by
     apply InvImage.wf
     exact WellFoundedRelation.wf
   subrelation {it it'} h := by
-    obtain ⟨step, hs, h⟩ := h
-    obtain ⟨step', hs', h'⟩ := LawfulMonadAttach.canReturn_bind_imp' h
-    cases step', hs' using PlausibleIterStep.casesOn'
-    · obtain ⟨Px, hPx, h'⟩ := LawfulMonadAttach.canReturn_bind_imp' h'
-      cases LawfulMonadAttach.eq_of_canReturn_pure h'
-      split at hs
-      · cases hs
-        exact IterM.TerminationMeasures.Finite.rel_of_yield ‹_›
-      · cases hs
-    · cases LawfulMonadAttach.eq_of_canReturn_pure h'
-      cases hs
-      exact IterM.TerminationMeasures.Finite.rel_of_skip ‹_›
-    · cases LawfulMonadAttach.eq_of_canReturn_pure h'
-      cases hs
+    obtain ⟨step, h, h'⟩ := h
+    cases h'
+    case yield it' out k h' h'' =>
+      cases h
+      exact IterM.TerminationMeasures.Finite.rel_of_yield h'
+    case skip it' out h' =>
+      cases h
+      exact IterM.TerminationMeasures.Finite.rel_of_skip h'
+    case done _ =>
+      cases h
+    case rejected _ =>
+      cases h
 
-instance TakeWhile.instFinite
-    [Monad m] [MonadAttach m] [LawfulMonad m] [LawfulMonadAttach m]
-    [Iterator α m β] [Finite α m] {P} :
+instance TakeWhile.instFinite [Monad m] [Iterator α m β] [Finite α m] {P} :
     Finite (TakeWhile α m β P) m :=
   by exact Finite.of_finitenessRelation instFinitenessRelation
 
-private def TakeWhile.instProductivenessRelation
-    [Monad m] [MonadAttach m] [LawfulMonad m] [LawfulMonadAttach m]
-    [Iterator α m β] [Productive α m] {P} :
+private def TakeWhile.instProductivenessRelation [Monad m] [Iterator α m β]
+    [Productive α m] {P} :
     ProductivenessRelation (TakeWhile α m β P) m where
   rel := InvImage WellFoundedRelation.rel (IterM.finitelyManySkips ∘ TakeWhile.inner ∘ IterM.internalState)
   wf := by
     apply InvImage.wf
     exact WellFoundedRelation.wf
   subrelation {it it'} h := by
-    obtain ⟨step, hs, h⟩ := LawfulMonadAttach.canReturn_bind_imp' h
-    cases step, hs using PlausibleIterStep.casesOn'
-    · obtain ⟨Px, hPx, h⟩ := LawfulMonadAttach.canReturn_bind_imp' h
-      have := LawfulMonadAttach.eq_of_canReturn_pure h
-      split at this <;> cases this
-    · cases LawfulMonadAttach.eq_of_canReturn_pure h
-      exact IterM.TerminationMeasures.Productive.rel_of_skip ‹_›
-    · cases LawfulMonadAttach.eq_of_canReturn_pure h
+    cases h
+    exact IterM.TerminationMeasures.Productive.rel_of_skip ‹_›
 
-instance TakeWhile.instProductive
-    [Monad m] [MonadAttach m] [LawfulMonad m] [LawfulMonadAttach m]
-    [Iterator α m β] [Productive α m] {P} :
+instance TakeWhile.instProductive [Monad m] [Iterator α m β] [Productive α m] {P} :
     Productive (TakeWhile α m β P) m :=
   by exact Productive.of_productivenessRelation instProductivenessRelation
 
-instance TakeWhile.instIteratorCollect
-    [Monad m] [MonadAttach m] [Monad n]
-    [Iterator α m β] [Productive α m] {P} :
+instance TakeWhile.instIteratorCollect [Monad m] [Monad n] [Iterator α m β] [Productive α m] {P} :
     IteratorCollect (TakeWhile α m β P) m n :=
   .defaultImplementation
 
-instance TakeWhile.instIteratorLoop
-    [Monad m] [MonadAttach m] [Monad n] [MonadAttach n]
-    [Iterator α m β] [IteratorLoop α m n] :
+instance TakeWhile.instIteratorLoop [Monad m] [Monad n] [Iterator α m β]
+    [IteratorLoop α m n] :
     IteratorLoop (TakeWhile α m β P) m n :=
   .defaultImplementation
 
